theories/Math/ClassicalCardinal.v
@@ -1,0 +1,1803 @@
+Require Import PnV.Prelude.Prelude.
+Require Import PnV.Math.OrderTheory.
+Require Import PnV.Data.Aczel.
+Require Import PnV.Prelude.ClassicalFacts.
+Require Import PnV.Math.SetTheory.
+Require Import PnV.Data.Vector.
+Require Import PnV.Math.ThN.
+Require Import PnV.Prelude.PnVTacs.
+Require Export PnV.Math.ClassicalSetTheory.
+
+Import TypeTheoreticImplementation.
+
+Module Cardinal3.
+
+Section CARDINALITY.
+
+Context `{Axms : ClassicalAxioms (b_AC := true) (b_fun_ext := true) (b_prop_ext := true)}.
+
+#[local] Existing Instance Aczel.children_isSetoid.
+
+Lemma Cardinality_ofType_bool_le_of_nat_le (A : Type@{Set_u})
+  (NAT_LE : Cardinality.ofType nat =< Cardinality.ofType A)
+  : Cardinality.ofType bool =< Cardinality.ofType A.
+Proof.
+  destruct NAT_LE as [f f_cong f_inj].
+  eapply Cardinal2.Cardinality_ofType_le_ofType with (f := fun b : bool => if b then f O else f (S O)).
+  intros [ | ] [ | ] EQ; try reflexivity.
+  - pose proof (f_inj O (S O) EQ) as H. discriminate H.
+  - pose proof (f_inj (S O) O EQ) as H. discriminate H.
+Qed.
+
+Definition option_pair_code {A : Type@{Set_u}} (tag : nat -> A) (pair : A * A -> A) (xy : option A * option A) : A :=
+  match xy with
+  | (None, None) => pair (tag O, tag O)
+  | (None, Some y) => pair (tag (S O), y)
+  | (Some x, None) => pair (tag (S (S O)), x)
+  | (Some x, Some y) => pair (tag (S (S (S O))), pair (x, y))
+  end.
+
+Lemma option_pair_code_inj {A : Type@{Set_u}} (tag : nat -> A) (pair : A * A -> A)
+  (TAG_INJ : forall n : nat, forall m : nat, tag n = tag m -> n = m)
+  (PAIR_INJ : forall p : A * A, forall q : A * A, pair p = pair q -> p = q)
+  : forall p : option A * option A, forall q : option A * option A, option_pair_code tag pair p = option_pair_code tag pair q -> p = q.
+Proof.
+  intros [[x | ] [y | ]] [[x' | ] [y' | ]] EQ; unfold option_pair_code in EQ.
+  - pose proof (PAIR_INJ _ _ EQ) as EQ_pair. inv EQ_pair.
+    pose proof (PAIR_INJ _ _ H0) as EQ_xy. inv EQ_xy. reflexivity.
+  - pose proof (PAIR_INJ _ _ EQ) as EQ_pair. inv EQ_pair.
+    pose proof (TAG_INJ (S (S (S O))) (S (S O)) H0) as Htag. discriminate Htag.
+  - pose proof (PAIR_INJ _ _ EQ) as EQ_pair. inv EQ_pair.
+    pose proof (TAG_INJ (S (S (S O))) (S O) H0) as Htag. discriminate Htag.
+  - pose proof (PAIR_INJ _ _ EQ) as EQ_pair. inv EQ_pair.
+    pose proof (TAG_INJ (S (S (S O))) O H0) as Htag. discriminate Htag.
+  - pose proof (PAIR_INJ _ _ EQ) as EQ_pair. inv EQ_pair.
+    pose proof (TAG_INJ (S (S O)) (S (S (S O))) H0) as Htag. discriminate Htag.
+  - pose proof (PAIR_INJ _ _ EQ) as EQ_pair. inv EQ_pair. reflexivity.
+  - pose proof (PAIR_INJ _ _ EQ) as EQ_pair. inv EQ_pair.
+    pose proof (TAG_INJ (S (S O)) (S O) H0) as Htag. discriminate Htag.
+  - pose proof (PAIR_INJ _ _ EQ) as EQ_pair. inv EQ_pair.
+    pose proof (TAG_INJ (S (S O)) O H0) as Htag. discriminate Htag.
+  - pose proof (PAIR_INJ _ _ EQ) as EQ_pair. inv EQ_pair.
+    pose proof (TAG_INJ (S O) (S (S (S O))) H0) as Htag. discriminate Htag.
+  - pose proof (PAIR_INJ _ _ EQ) as EQ_pair. inv EQ_pair.
+    pose proof (TAG_INJ (S O) (S (S O)) H0) as Htag. discriminate Htag.
+  - pose proof (PAIR_INJ _ _ EQ) as EQ_pair. inv EQ_pair. reflexivity.
+  - pose proof (PAIR_INJ _ _ EQ) as EQ_pair. inv EQ_pair.
+    pose proof (TAG_INJ (S O) O H0) as Htag. discriminate Htag.
+  - pose proof (PAIR_INJ _ _ EQ) as EQ_pair. inv EQ_pair.
+    pose proof (TAG_INJ O (S (S (S O))) H0) as Htag. discriminate Htag.
+  - pose proof (PAIR_INJ _ _ EQ) as EQ_pair. inv EQ_pair.
+    pose proof (TAG_INJ O (S (S O)) H0) as Htag. discriminate Htag.
+  - pose proof (PAIR_INJ _ _ EQ) as EQ_pair. inv EQ_pair.
+    pose proof (TAG_INJ O (S O) H0) as Htag. discriminate Htag.
+  - pose proof (PAIR_INJ _ _ EQ) as EQ_pair. inv EQ_pair. reflexivity.
+Qed.
+
+Lemma Cardinality_ofType_option_prod_le_self_of_nat_le_square_le (A : Type@{Set_u})
+  (NAT_LE : Cardinality.ofType nat =< Cardinality.ofType A)
+  (SQUARE_LE : Cardinality.ofType (A * A) =< Cardinality.ofType A)
+  : Cardinality.ofType (option A * option A) =< Cardinality.ofType A.
+Proof.
+  destruct NAT_LE as [tag tag_cong tag_inj]. destruct SQUARE_LE as [pair pair_cong pair_inj].
+  eapply Cardinal2.Cardinality_ofType_le_ofType with (f := option_pair_code tag pair).
+  eapply option_pair_code_inj.
+  - intros n m EQ. change (n = m). eapply tag_inj. change (tag n = tag m). exact EQ.
+  - intros [x y] [x' y'] EQ. change ((x, y) = (x', y')). eapply pair_inj. change (pair (x, y) = pair (x', y')). exact EQ.
+Qed.
+
+Fixpoint encode_list_by_pair {A : Type@{Set_u}} (pair : A * A -> A) (pack : option A -> A) (xs : list A) : option A :=
+  match xs with
+  | [] => None
+  | x :: xs => Some (pair (x, pack (encode_list_by_pair pair pack xs)))
+  end.
+
+Lemma encode_list_by_pair_inj {A : Type@{Set_u}} (pair : A * A -> A) (pack : option A -> A)
+  (PAIR_INJ : forall p : A * A, forall q : A * A, pair p = pair q -> p = q)
+  (PACK_INJ : forall x : option A, forall y : option A, pack x = pack y -> x = y)
+  : forall xs : list A, forall ys : list A, encode_list_by_pair pair pack xs = encode_list_by_pair pair pack ys -> xs = ys.
+Proof.
+  induction xs as [ | x xs IH]; intros [ | y ys] EQ; simpl in EQ.
+  - reflexivity.
+  - discriminate EQ.
+  - discriminate EQ.
+  - injection EQ as EQ_code. pose proof (PAIR_INJ _ _ EQ_code) as EQ_pair.
+    injection EQ_pair as EQ_x EQ_pack. subst y. f_equal. eapply IH. eapply PACK_INJ. exact EQ_pack.
+Qed.
+
+Lemma Cardinality_ofType_list_le_self_of_nat_le_square_le (A : Type@{Set_u})
+  (NAT_LE : Cardinality.ofType nat =< Cardinality.ofType A)
+  (SQUARE_LE : Cardinality.ofType (A * A) =< Cardinality.ofType A)
+  : Cardinality.ofType (list A) =< Cardinality.ofType A.
+Proof.
+  destruct SQUARE_LE as [pair pair_cong pair_inj].
+  pose proof (Cardinal2.Cardinality_ofType_option_le_self_of_nat_le A NAT_LE) as OPTION_LE.
+  pose proof OPTION_LE as OPTION_LE'.
+  destruct OPTION_LE as [pack pack_cong pack_inj].
+  transitivity (Cardinality.ofType (option A)).
+  - eapply Cardinal2.Cardinality_ofType_le_ofType with (f := encode_list_by_pair pair pack).
+    eapply encode_list_by_pair_inj.
+    + intros [x y] [x' y'] EQ. change ((x, y) = (x', y')). eapply pair_inj. change (pair (x, y) = pair (x', y')). exact EQ.
+    + intros x y EQ. change (x = y). eapply pack_inj. change (pack x = pack y). exact EQ.
+  - exact OPTION_LE'.
+Qed.
+
+Lemma Cardinality_ofType_sum_nat_le_self_of_nat_le_square_le (A : Type@{Set_u})
+  (NAT_LE : Cardinality.ofType nat =< Cardinality.ofType A)
+  (SQUARE_LE : Cardinality.ofType (A * A) =< Cardinality.ofType A)
+  : Cardinality.ofType (A + nat) =< Cardinality.ofType A.
+Proof.
+  transitivity (Cardinality.ofType (bool * A)).
+  - destruct NAT_LE as [tag tag_cong tag_inj].
+    eapply Cardinal2.Cardinality_ofType_le_ofType with (f := fun x : A + nat => match x with inl a => (true, a) | inr n => (false, tag n) end).
+    intros [a | n] [a' | n'] EQ; simpl in EQ.
+    + inv EQ. reflexivity.
+    + inv EQ.
+    + inv EQ.
+    + injection EQ as EQ_tag. f_equal. eapply tag_inj. exact EQ_tag.
+  - transitivity (Cardinality.ofType (A * A)).
+    + eapply Cardinal2.Cardinality_ofType_prod_le.
+      * eapply Cardinality_ofType_bool_le_of_nat_le. exact NAT_LE.
+      * reflexivity.
+    + exact SQUARE_LE.
+Qed.
+
+Lemma Cardinality_ofType_list_sum_nat_le_self_of_nat_le_square_le (A : Type@{Set_u})
+  (NAT_LE : Cardinality.ofType nat =< Cardinality.ofType A)
+  (SQUARE_LE : Cardinality.ofType (A * A) =< Cardinality.ofType A)
+  : Cardinality.ofType (list (A + nat)) =< Cardinality.ofType A.
+Proof.
+  transitivity (Cardinality.ofType (list A)).
+  - eapply Cardinal2.Cardinality_ofType_list_le.
+    eapply Cardinality_ofType_sum_nat_le_self_of_nat_le_square_le; eauto.
+  - eapply Cardinality_ofType_list_le_self_of_nat_le_square_le; eauto.
+Qed.
+
+Lemma Cardinality_ofType_rose_le_self_of_nat_le_square_le (A : Type@{Set_u})
+  (NAT_LE : Cardinality.ofType nat =< Cardinality.ofType A)
+  (SQUARE_LE : Cardinality.ofType (A * A) =< Cardinality.ofType A)
+  : Cardinality.ofType (B.rose A) =< Cardinality.ofType A.
+Proof.
+  transitivity (Cardinality.ofType (list (A + nat))).
+  - eapply Cardinal2.Cardinality_ofType_rose_le_list_sum_nat.
+  - eapply Cardinality_ofType_list_sum_nat_le_self_of_nat_le_square_le; eauto.
+Qed.
+
+Lemma Cardinality_ofType_rose_lt_of_lt_uncountable_square_le (A : Type@{Set_u}) (kappa : Cardinality.t)
+  (LT : Cardinality.ofType A ≨ kappa)
+  (UNCOUNTABLE : ~ kappa =< Cardinality.ofType nat)
+  (SQUARE : forall B : Type@{Set_u}, Cardinality.ofType nat =< Cardinality.ofType B -> Cardinality.ofType (B * B) =< Cardinality.ofType B)
+  : Cardinality.ofType (B.rose A) ≨ kappa.
+Proof.
+  pose proof (Cardinal1.Cardinality_le_total (Cardinality.ofType A) (Cardinality.ofType nat)) as [A_LE_NAT | NAT_LE_A].
+  - eapply Cardinal1.Cardinality_le_lt_lt.
+    + transitivity (Cardinality.ofType (list (nat + nat))).
+      * destruct A_LE_NAT as [f f_cong f_inj].
+        eapply Cardinal2.Cardinality_ofType_le_ofType with (f := fun t : B.rose A => map (fun x : A + nat => match x with inl a => inl (f a) | inr n => inr n end) (Cardinal2.encode_rose t)).
+        intros t1 t2 EQ. eapply Cardinal2.encode_rose_inj. apply L.list_map_inj in EQ.
+        { exact EQ. }
+        intros [a | n] [a' | n'] EQ'; inv EQ'.
+        { f_equal. eapply f_inj. exact H0. }
+        { reflexivity. }
+      * eapply Cardinal2.Cardinality_ofType_list_countable_le_nat.
+    + eapply Cardinal2.nat_lt_of_uncountable. exact UNCOUNTABLE.
+  - eapply Cardinal1.Cardinality_le_lt_lt.
+    + eapply Cardinality_ofType_rose_le_self_of_nat_le_square_le.
+      * exact NAT_LE_A.
+      * eapply SQUARE. exact NAT_LE_A.
+    + exact LT.
+Qed.
+
+Theorem Cardinality_ofType_rank_strict_initial_segment_lt (A : Type@{Set_u}) (kappa : Ord.t)
+  (K_CARD : Cardinal1.hasCardinality (Cardinality.ofType A) kappa)
+  (enum : Aczel.children kappa -> A)
+  (enum_inj : forall c1 : Aczel.children kappa, forall c2 : Aczel.children kappa, c1 == c2 <-> enum c1 = enum c2)
+  (rank : A -> Aczel.children kappa)
+  (RANK : forall x : A, enum (rank x) = x)
+  : forall a : A, Cardinality.ofType { x : A | Aczel.isElemOf kappa (rank x) (rank a) } ≨ Cardinality.ofType A.
+Proof.
+  i.
+  pose proof (Cardinal1.hasCardinality_isOrdinal _ _ K_CARD) as K_ORD.
+  set (alpha := Aczel.childnodes kappa (rank a)).
+  assert (ALPHA_ORD : Aczel.isOrdinal alpha).
+  { eapply Aczel.isOrdinal_member_isOrdinal.
+    - exact K_ORD.
+    - unfold alpha. eapply Aczel.member_intro.
+  }
+  assert (ALPHA_LT : alpha <ᵣ kappa).
+  { unfold alpha. eapply Aczel.member_implies_rLt. eapply Aczel.member_intro. }
+  assert (STRICT_LE : Cardinality.ofType { x : A | Aczel.isElemOf kappa (rank x) (rank a) } =< card alpha).
+  { assert (Hchoice : forall i : { x : A | Aczel.isElemOf kappa (rank x) (rank a) }, exists c : Aczel.children alpha, Aczel.childnodes alpha c == Aczel.childnodes kappa (rank (proj1_sig i))).
+    { intros [x Hx]. unfold alpha. unfold Aczel.isElemOf in Hx. destruct Hx as [c EQ]. exists c. symmetry. exact EQ. }
+    pose proof (Axiom_of_Choice { x : A | Aczel.isElemOf kappa (rank x) (rank a) } (fun _ : { x : A | Aczel.isElemOf kappa (rank x) (rank a) } => Aczel.children alpha) (fun i : { x : A | Aczel.isElemOf kappa (rank x) (rank a) } => fun c : Aczel.children alpha => Aczel.childnodes alpha c == Aczel.childnodes kappa (rank (proj1_sig i))) Hchoice) as [pick PICK].
+    exists pick.
+    - intros i j EQ. change (i = j) in EQ. subst j. reflexivity.
+    - intros [x Hx] [y Hy] EQ. eapply Cardinal2.sig_eq_from_proj1. simpl.
+      assert (RANK_EQ : rank x == rank y).
+      { change (Aczel.childnodes kappa (rank x) == Aczel.childnodes kappa (rank y)).
+        transitivity (Aczel.childnodes alpha (pick (@exist A (fun z : A => Aczel.isElemOf kappa (rank z) (rank a)) x Hx))).
+        - symmetry. exact (PICK (@exist A (fun z : A => Aczel.isElemOf kappa (rank z) (rank a)) x Hx)).
+        - transitivity (Aczel.childnodes alpha (pick (@exist A (fun z : A => Aczel.isElemOf kappa (rank z) (rank a)) y Hy))).
+          + exact EQ.
+          + exact (PICK (@exist A (fun z : A => Aczel.isElemOf kappa (rank z) (rank a)) y Hy)).
+      }
+      pose proof (proj1 (enum_inj (rank x) (rank y)) RANK_EQ) as ENUM_EQ. now rewrite 2 RANK in ENUM_EQ.
+  }
+  assert (K_CARDINAL : Cardinal1.isCardinal kappa).
+  { exists (Cardinality.ofType A). exact K_CARD. }
+  pose proof (Cardinal1.card_children_lt_card_of_rLt alpha kappa ALPHA_ORD K_CARDINAL ALPHA_LT) as CARD_ALPHA_LT_KAPPA.
+  assert (CARD_KAPPA_LE : card kappa =< Cardinality.ofType A).
+  { pose proof (Cardinal1.isCardinal_elim kappa K_CARDINAL) as CARD_KAPPA.
+    rewrite Cardinal1.Cardinality_le_iff. rewrite (Cardinal1.Cardinality_toTree_eq_intro (card kappa) kappa CARD_KAPPA).
+    rewrite (Cardinal1.Cardinality_toTree_eq_intro (Cardinality.ofType A) kappa K_CARD). reflexivity.
+  }
+  eapply Cardinal1.Cardinality_le_lt_lt.
+  - exact STRICT_LE.
+  - eapply Cardinal1.Cardinality_lt_le_lt.
+    + exact CARD_ALPHA_LT_KAPPA.
+    + exact CARD_KAPPA_LE.
+Qed.
+
+Theorem Cardinality_ofType_rank_initial_segment_lt (A : Type@{Set_u}) (kappa : Ord.t)
+  (K_CARD : Cardinal1.hasCardinality (Cardinality.ofType A) kappa)
+  (UNCOUNTABLE : ~ Cardinality.ofType A =< Cardinality.ofType nat)
+  (enum : Aczel.children kappa -> A)
+  (enum_inj : forall c1 : Aczel.children kappa, forall c2 : Aczel.children kappa, c1 == c2 <-> enum c1 = enum c2)
+  (rank : A -> Aczel.children kappa)
+  (RANK : forall x : A, enum (rank x) = x)
+  : forall a : A, Cardinality.ofType { x : A | Aczel.isElemOf kappa (rank x) (rank a) \/ Aczel.eqTree (Aczel.childnodes kappa (rank x)) (Aczel.childnodes kappa (rank a)) } ≨ Cardinality.ofType A.
+Proof.
+  i.
+  set (StrictIdx := { x : A | Aczel.isElemOf kappa (rank x) (rank a) }).
+  set (Idx := { x : A | Aczel.isElemOf kappa (rank x) (rank a) \/ Aczel.eqTree (Aczel.childnodes kappa (rank x)) (Aczel.childnodes kappa (rank a)) }).
+  assert (IDX_LE : Cardinality.ofType Idx =< Cardinality.ofType (option StrictIdx)).
+  { assert (Hchoice : forall i : Idx, exists oi : option StrictIdx, match oi with | Some j => proj1_sig j = proj1_sig i | None => rank (proj1_sig i) == rank a end).
+    { intros [x [LT | EQ]].
+      - exists (Some (@exist A (fun z : A => Aczel.isElemOf kappa (rank z) (rank a)) x LT)). reflexivity.
+      - exists None. exact EQ.
+    }
+    pose proof (Axiom_of_Choice Idx (fun _ : Idx => option StrictIdx) (fun i : Idx => fun oi : option StrictIdx => match oi with | Some j => proj1_sig j = proj1_sig i | None => rank (proj1_sig i) == rank a end) Hchoice) as [pick PICK].
+    exists pick.
+    - intros i j EQ. change (i = j) in EQ. subst j. reflexivity.
+    - intros [x Hx] [y Hy] EQ. unfold Idx in *. simpl in *.
+      pose proof (PICK (@exist A (fun z : A => Aczel.isElemOf kappa (rank z) (rank a) \/ Aczel.eqTree (Aczel.childnodes kappa (rank z)) (Aczel.childnodes kappa (rank a))) x Hx)) as PICKx.
+      pose proof (PICK (@exist A (fun z : A => Aczel.isElemOf kappa (rank z) (rank a) \/ Aczel.eqTree (Aczel.childnodes kappa (rank z)) (Aczel.childnodes kappa (rank a))) y Hy)) as PICKy.
+      destruct (pick (@exist A (fun z : A => Aczel.isElemOf kappa (rank z) (rank a) \/ Aczel.eqTree (Aczel.childnodes kappa (rank z)) (Aczel.childnodes kappa (rank a))) x Hx)) as [[x' Hx'] | ] eqn:PICK_X; destruct (pick (@exist A (fun z : A => Aczel.isElemOf kappa (rank z) (rank a) \/ Aczel.eqTree (Aczel.childnodes kappa (rank z)) (Aczel.childnodes kappa (rank a))) y Hy)) as [[y' Hy'] | ] eqn:PICK_Y; simpl in *.
+      + injection EQ as STRICT_EQ. eapply Cardinal2.sig_eq_from_proj1. simpl.
+        rewrite <- PICKx. rewrite <- PICKy. exact STRICT_EQ.
+      + discriminate EQ.
+      + discriminate EQ.
+      + eapply Cardinal2.sig_eq_from_proj1. simpl.
+        assert (RANK_EQ : rank x == rank y).
+        { transitivity (rank a); [exact PICKx | symmetry; exact PICKy]. }
+        pose proof (proj1 (enum_inj (rank x) (rank y)) RANK_EQ) as ENUM_EQ. now rewrite 2 RANK in ENUM_EQ.
+  }
+  eapply Cardinal1.Cardinality_le_lt_lt.
+  - unfold Idx in IDX_LE. exact IDX_LE.
+  - eapply Cardinal2.Cardinality_ofType_option_lt_of_lt_uncountable.
+    + unfold StrictIdx. eapply Cardinality_ofType_rank_strict_initial_segment_lt; eauto.
+    + exact UNCOUNTABLE.
+Qed.
+
+Section SQUARE_ABSORPTION.
+
+Variable A : Type@{Set_u}.
+
+Variable nat_embed : nat -> A.
+
+Hypothesis nat_embed_inj : forall n : nat, forall m : nat, nat_embed n = nat_embed m -> n = m.
+
+Record square_state : Type :=
+  mk_square_state
+  { st_carrier : Type@{Set_u}
+  ; st_isSetoid : isSetoid st_carrier
+  ; st_emb : st_carrier -> A
+  ; st_emb_cong : forall x : st_carrier, forall y : st_carrier, @eqProp st_carrier st_isSetoid x y -> st_emb x = st_emb y
+  ; st_emb_inj : forall x : st_carrier, forall y : st_carrier, st_emb x = st_emb y -> @eqProp st_carrier st_isSetoid x y
+  ; st_nat : nat -> st_carrier
+  ; st_nat_emb : forall n : nat, st_emb (st_nat n) = nat_embed n
+  ; st_code : st_carrier * st_carrier -> st_carrier
+  ; st_code_cong : forall x1 : st_carrier, forall x2 : st_carrier, forall y1 : st_carrier, forall y2 : st_carrier, @eqProp st_carrier st_isSetoid x1 x2 -> @eqProp st_carrier st_isSetoid y1 y2 -> @eqProp st_carrier st_isSetoid (st_code (x1, y1)) (st_code (x2, y2))
+  ; st_code_inj : forall x1 : st_carrier, forall x2 : st_carrier, forall y1 : st_carrier, forall y2 : st_carrier, @eqProp st_carrier st_isSetoid (st_code (x1, y1)) (st_code (x2, y2)) -> @eqProp st_carrier st_isSetoid x1 x2 /\ @eqProp st_carrier st_isSetoid y1 y2
+  }.
+
+Definition state_card (s : square_state) : Cardinality.t :=
+  Cardinality.mk (st_carrier s) (st_isSetoid s).
+
+Lemma st_nat_inj (s : square_state) (n : nat) (m : nat)
+  (EQ : @eqProp (st_carrier s) (st_isSetoid s) (st_nat s n) (st_nat s m))
+  : n = m.
+Proof.
+  eapply nat_embed_inj. rewrite <- (st_nat_emb s n). rewrite <- (st_nat_emb s m). now eapply st_emb_cong.
+Qed.
+
+Definition square_state_initial
+  : square_state.
+Proof.
+  refine (
+    {|
+      st_carrier := nat;
+      st_isSetoid := mkSetoid_from_eq;
+      st_emb := nat_embed;
+      st_emb_cong := _;
+      st_emb_inj := _;
+      st_nat := fun n : nat => n;
+      st_nat_emb := fun _ : nat => eq_refl;
+      st_code := fun xy : nat * nat => cpInv (Datatypes.fst xy) (Datatypes.snd xy);
+      st_code_cong := _;
+      st_code_inj := _;
+    |}
+  ).
+  - intros x y EQ. change (x = y) in EQ. subst y. reflexivity.
+  - intros x y EQ. eapply nat_embed_inj. exact EQ.
+  - intros x1 x2 y1 y2 EQ_x EQ_y. change (x1 = x2) in EQ_x. change (y1 = y2) in EQ_y. now subst x2 y2.
+  - intros x1 x2 y1 y2 EQ. eapply cpInv_inj. exact EQ.
+Defined.
+
+Record state_embedding (s : square_state) (t : square_state) : Type :=
+  mk_state_embedding
+  { st_lift : st_carrier s -> st_carrier t
+  ; st_lift_cong : forall x : st_carrier s, forall y : st_carrier s, @eqProp (st_carrier s) (st_isSetoid s) x y -> @eqProp (st_carrier t) (st_isSetoid t) (st_lift x) (st_lift y)
+  ; st_lift_emb : forall x : st_carrier s, st_emb t (st_lift x) = st_emb s x
+  ; st_lift_code : forall x : st_carrier s, forall y : st_carrier s, @eqProp (st_carrier t) (st_isSetoid t) (st_lift (st_code s (x, y))) (st_code t (st_lift x, st_lift y))
+  }.
+
+Definition state_le (s : square_state) (t : square_state) : Prop :=
+  exists emb : state_embedding s t, True.
+
+#[local]
+Instance state_le_PreOrder
+  : PreOrder state_le.
+Proof.
+  split.
+  - intros s.
+    exists (
+      {|
+        st_lift := fun x : st_carrier s => x;
+        st_lift_cong := fun _ => fun _ => fun H => H;
+        st_lift_emb := fun _ => eq_refl;
+        st_lift_code := fun _ => fun _ => eqProp_refl _;
+      |}
+    ).
+    exact I.
+  - intros s t u [emb_st _] [emb_tu _].
+    unshelve eexists (
+      {|
+        st_lift := fun x : st_carrier s => st_lift t u emb_tu (st_lift s t emb_st x);
+        st_lift_cong := fun x => fun y => fun H => st_lift_cong t u emb_tu _ _ (st_lift_cong s t emb_st _ _ H);
+        st_lift_emb := _;
+        st_lift_code := _;
+      |}
+    ); [simpl | simpl | exact I].
+    + intros x. rewrite st_lift_emb. eapply st_lift_emb.
+    + intros x y. transitivity (st_lift t u emb_tu (st_code t (st_lift s t emb_st x, st_lift s t emb_st y))).
+      * eapply st_lift_cong. eapply st_lift_code.
+      * eapply st_lift_code.
+Qed.
+
+#[local]
+Instance square_state_isProset : isProset square_state :=
+  { leProp := state_le
+  ; Proset_isSetoid := mkSetoidFromPreOrder state_le_PreOrder
+  ; leProp_PreOrder := state_le_PreOrder
+  ; leProp_PartialOrder := mkSetoidFromPreOrder_good state_le_PreOrder
+  }.
+
+Definition state_encode_sum (s : square_state) (x : st_carrier s + st_carrier s) : st_carrier s :=
+  match x with
+  | inl a => st_code s (st_nat s O, a)
+  | inr a => st_code s (st_nat s (S O), a)
+  end.
+
+Definition state_sum_isSetoid (s : square_state) : isSetoid (st_carrier s + st_carrier s) :=
+  @sum_isSetoid (st_carrier s) (st_carrier s) (st_isSetoid s) (st_isSetoid s).
+
+Definition state_sum_prod_isSetoid (s : square_state) : isSetoid ((st_carrier s + st_carrier s) * (st_carrier s + st_carrier s)) :=
+  @prod_isSetoid _ _ (state_sum_isSetoid s) (state_sum_isSetoid s).
+
+Lemma state_encode_sum_cong (s : square_state)
+  : forall x : st_carrier s + st_carrier s, forall y : st_carrier s + st_carrier s, @eqProp (st_carrier s + st_carrier s) (state_sum_isSetoid s) x y -> @eqProp (st_carrier s) (st_isSetoid s) (state_encode_sum s x) (state_encode_sum s y).
+Proof.
+  intros [x | x] [y | y] EQ; inv EQ; simpl.
+  - eapply st_code_cong; [reflexivity | exact x_corres].
+  - eapply st_code_cong; [reflexivity | exact y_corres].
+Qed.
+
+Lemma state_encode_sum_inj (s : square_state)
+  : forall x : st_carrier s + st_carrier s, forall y : st_carrier s + st_carrier s, @eqProp (st_carrier s) (st_isSetoid s) (state_encode_sum s x) (state_encode_sum s y) -> @eqProp (st_carrier s + st_carrier s) (state_sum_isSetoid s) x y.
+Proof.
+  intros [x | x] [y | y] EQ; simpl in EQ.
+  - pose proof (st_code_inj s (st_nat s O) (st_nat s O) x y EQ) as [_ EQ_xy]. econs. exact EQ_xy.
+  - pose proof (st_code_inj s (st_nat s O) (st_nat s (S O)) x y EQ) as [EQ_tag _].
+    pose proof (st_nat_inj s O (S O) EQ_tag) as BAD. discriminate BAD.
+  - pose proof (st_code_inj s (st_nat s (S O)) (st_nat s O) x y EQ) as [EQ_tag _].
+    pose proof (st_nat_inj s (S O) O EQ_tag) as BAD. discriminate BAD.
+  - pose proof (st_code_inj s (st_nat s (S O)) (st_nat s (S O)) x y EQ) as [_ EQ_xy]. econs. exact EQ_xy.
+Qed.
+
+Definition state_encode_pair (s : square_state) (xy : (st_carrier s + st_carrier s) * (st_carrier s + st_carrier s)) : st_carrier s :=
+  st_code s (state_encode_sum s (Datatypes.fst xy), state_encode_sum s (Datatypes.snd xy)).
+
+Lemma state_encode_pair_cong (s : square_state)
+  : forall p : (st_carrier s + st_carrier s) * (st_carrier s + st_carrier s), forall q : (st_carrier s + st_carrier s) * (st_carrier s + st_carrier s), @eqProp ((st_carrier s + st_carrier s) * (st_carrier s + st_carrier s)) (state_sum_prod_isSetoid s) p q -> @eqProp (st_carrier s) (st_isSetoid s) (state_encode_pair s p) (state_encode_pair s q).
+Proof.
+  intros [x1 y1] [x2 y2] [EQ_x EQ_y]. simpl.
+  eapply st_code_cong; eapply state_encode_sum_cong; assumption.
+Qed.
+
+Lemma state_encode_pair_inj (s : square_state)
+  : forall p : (st_carrier s + st_carrier s) * (st_carrier s + st_carrier s), forall q : (st_carrier s + st_carrier s) * (st_carrier s + st_carrier s), @eqProp (st_carrier s) (st_isSetoid s) (state_encode_pair s p) (state_encode_pair s q) -> @eqProp ((st_carrier s + st_carrier s) * (st_carrier s + st_carrier s)) (state_sum_prod_isSetoid s) p q.
+Proof.
+  intros [x1 y1] [x2 y2] EQ. simpl in EQ.
+  pose proof (st_code_inj s (state_encode_sum s x1) (state_encode_sum s x2) (state_encode_sum s y1) (state_encode_sum s y2) EQ) as [EQ_x EQ_y].
+  split; eapply state_encode_sum_inj; assumption.
+Qed.
+
+Definition square_state_extend (s : square_state) (fresh : st_carrier s -> A)
+  (fresh_cong : forall x : st_carrier s, forall y : st_carrier s, @eqProp (st_carrier s) (st_isSetoid s) x y -> fresh x = fresh y)
+  (fresh_inj : forall x : st_carrier s, forall y : st_carrier s, fresh x = fresh y -> @eqProp (st_carrier s) (st_isSetoid s) x y)
+  (fresh_out : forall x : st_carrier s, forall y : st_carrier s, ~ fresh x = st_emb s y)
+  : square_state.
+Proof.
+  pose (B := st_carrier s).
+  pose (B_isSetoid := st_isSetoid s).
+  refine (
+    {|
+      st_carrier := B + B;
+      st_isSetoid := @sum_isSetoid B B B_isSetoid B_isSetoid;
+      st_emb := fun x : B + B => match x with inl b => st_emb s b | inr b => fresh b end;
+      st_emb_cong := _;
+      st_emb_inj := _;
+      st_nat := fun n : nat => inl (st_nat s n);
+      st_nat_emb := _;
+      st_code := fun xy : (B + B) * (B + B) => match Datatypes.fst xy, Datatypes.snd xy with inl x, inl y => inl (st_code s (x, y)) | _, _ => inr (state_encode_pair s xy) end;
+      st_code_cong := _;
+      st_code_inj := _;
+    |}
+  ).
+  - intros [x | x] [y | y] EQ; inv EQ; simpl.
+    + eapply st_emb_cong. exact x_corres.
+    + eapply fresh_cong. exact y_corres.
+  - intros [x | x] [y | y] EQ; simpl in EQ.
+    + econs. eapply st_emb_inj. exact EQ.
+    + exfalso. exact (fresh_out y x (eq_sym EQ)).
+    + exfalso. exact (fresh_out x y EQ).
+    + econs. eapply fresh_inj. exact EQ.
+  - intros n. eapply st_nat_emb.
+  - intros [x1 | x1] [x2 | x2] [y1 | y1] [y2 | y2] EQ_x EQ_y; inv EQ_x; inv EQ_y; simpl.
+    + econs. eapply st_code_cong; eauto.
+    + econs. eapply state_encode_pair_cong. split; econs; eauto.
+    + econs. eapply state_encode_pair_cong. split; econs; eauto.
+    + econs. eapply state_encode_pair_cong. split; econs; eauto.
+  - intros [x1 | x1] [x2 | x2] [y1 | y1] [y2 | y2] EQ; simpl in EQ; inv EQ.
+    + pose proof (st_code_inj s x1 x2 y1 y2 x_corres) as [EQ_x EQ_y]. split; econs; assumption.
+    + pose proof (state_encode_pair_inj s _ _ y_corres) as [EQ_x EQ_y]. split; assumption.
+    + pose proof (state_encode_pair_inj s _ _ y_corres) as [EQ_x EQ_y]. split; assumption.
+    + pose proof (state_encode_pair_inj s _ _ y_corres) as [EQ_x EQ_y]. split; assumption.
+    + pose proof (state_encode_pair_inj s _ _ y_corres) as [EQ_x EQ_y]. split; assumption.
+    + pose proof (state_encode_pair_inj s _ _ y_corres) as [EQ_x EQ_y]. split; assumption.
+    + pose proof (state_encode_pair_inj s _ _ y_corres) as [EQ_x EQ_y]. split; assumption.
+    + pose proof (state_encode_pair_inj s _ _ y_corres) as [EQ_x EQ_y]. split; assumption.
+    + pose proof (state_encode_pair_inj s _ _ y_corres) as [EQ_x EQ_y]. split; assumption.
+    + pose proof (state_encode_pair_inj s _ _ y_corres) as [EQ_x EQ_y]. split; assumption.
+Defined.
+
+Lemma square_state_extend_exists (s : square_state) (fresh : st_carrier s -> A)
+  (fresh_cong : forall x : st_carrier s, forall y : st_carrier s, @eqProp (st_carrier s) (st_isSetoid s) x y -> fresh x = fresh y)
+  (fresh_inj : forall x : st_carrier s, forall y : st_carrier s, fresh x = fresh y -> @eqProp (st_carrier s) (st_isSetoid s) x y)
+  (fresh_out : forall x : st_carrier s, forall y : st_carrier s, ~ fresh x = st_emb s y)
+  : exists t : square_state, state_le s t.
+Proof.
+  exists (square_state_extend s fresh fresh_cong fresh_inj fresh_out).
+  unfold state_le. cbn. eexists; [change (state_embedding s (square_state_extend s fresh fresh_cong fresh_inj fresh_out)) | exact I].
+  unshelve refine (
+    {|
+      st_lift := fun x : st_carrier s => (inl x : st_carrier (square_state_extend s fresh fresh_cong fresh_inj fresh_out));
+      st_lift_cong := _;
+      st_lift_emb := _;
+      st_lift_code := _;
+    |}
+  ).
+  - intros x y H. econs. exact H.
+  - intros x. reflexivity.
+  - intros x y. reflexivity.
+Qed.
+
+End SQUARE_ABSORPTION.
+
+Section GRAPH_SQUARE_ABSORPTION.
+
+#[local] Infix "\in" := E.In : type_scope.
+
+Variable A : Type@{Set_u}.
+
+Variable nat_embed : nat -> A.
+
+Hypothesis nat_embed_inj : forall n : nat, forall m : nat, nat_embed n = nat_embed m -> n = m.
+
+Record graph_state : Type@{Set_u} :=
+  mk_graph_state
+  { gs_carrier : A -> Prop
+  ; gs_nat : forall n : nat, gs_carrier (nat_embed n)
+  ; gs_code : A -> A -> A -> Prop
+  ; gs_code_dom : forall x : A, forall y : A, forall z : A, gs_code x y z -> gs_carrier x /\ gs_carrier y /\ gs_carrier z
+  ; gs_code_total : forall x : A, forall y : A, gs_carrier x -> gs_carrier y -> exists z : A, gs_code x y z
+  ; gs_code_functional : forall x : A, forall y : A, forall z1 : A, forall z2 : A, gs_code x y z1 -> gs_code x y z2 -> z1 = z2
+  ; gs_code_inj : forall x1 : A, forall y1 : A, forall z1 : A, forall x2 : A, forall y2 : A, forall z2 : A, gs_code x1 y1 z1 -> gs_code x2 y2 z2 -> z1 = z2 -> x1 = x2 /\ y1 = y2
+  }.
+
+Definition graph_state_le (s : graph_state) (t : graph_state) : Prop :=
+  (forall a : A, gs_carrier s a -> gs_carrier t a) /\ (forall x : A, forall y : A, forall z : A, gs_code s x y z -> gs_code t x y z).
+
+#[local]
+Instance graph_state_le_PreOrder
+  : PreOrder graph_state_le.
+Proof.
+  split.
+  - intros s. split; eauto.
+  - intros s t u LE_st LE_tu. split.
+    + intros a Ha. exact (proj1 LE_tu a (proj1 LE_st a Ha)).
+    + intros x y z Hcode. exact (proj2 LE_tu x y z (proj2 LE_st x y z Hcode)).
+Qed.
+
+#[local]
+Instance graph_state_isProset : isProset graph_state :=
+  { leProp := graph_state_le
+  ; Proset_isSetoid := mkSetoidFromPreOrder graph_state_le_PreOrder
+  ; leProp_PreOrder := graph_state_le_PreOrder
+  ; leProp_PartialOrder := mkSetoidFromPreOrder_good graph_state_le_PreOrder
+  }.
+
+Definition graph_state_initial_code (x : A) (y : A) (z : A) : Prop :=
+  exists n : nat, exists m : nat, x = nat_embed n /\ y = nat_embed m /\ z = nat_embed (cpInv n m).
+
+Definition graph_state_initial
+  : graph_state.
+Proof.
+  refine (
+    {|
+      gs_carrier := fun a : A => exists n : nat, a = nat_embed n;
+      gs_nat := _;
+      gs_code := graph_state_initial_code;
+      gs_code_dom := _;
+      gs_code_total := _;
+      gs_code_functional := _;
+      gs_code_inj := _;
+    |}
+  ).
+  - intros n. exists n. reflexivity.
+  - intros x y z (n & m & Hx & Hy & Hz). subst. splits; eauto.
+  - intros x y (n & Hx) (m & Hy). subst. exists (nat_embed (cpInv n m)). exists n, m. splits; reflexivity.
+  - intros x y z1 z2 (n1 & m1 & Hx1 & Hy1 & Hz1) (n2 & m2 & Hx2 & Hy2 & Hz2). subst.
+    assert (n1 = n2) by now eapply nat_embed_inj.
+    assert (m1 = m2) by now eapply nat_embed_inj.
+    now subst n2 m2.
+  - intros x1 y1 z1 x2 y2 z2 (n1 & m1 & Hx1 & Hy1 & Hz1) (n2 & m2 & Hx2 & Hy2 & Hz2) Hz. subst.
+    pose proof (nat_embed_inj _ _ Hz) as Hpair. pose proof (cpInv_inj _ _ _ _ Hpair) as [Hn Hm]. subst n2 m2. split; reflexivity.
+Defined.
+
+Definition graph_state_chain_upperbound (C : ensemble graph_state)
+  (NONEMPTY : exists s : graph_state, s \in C)
+  (CHAIN : forall s1 : graph_state, forall s2 : graph_state, s1 \in C -> s2 \in C -> graph_state_le s1 s2 \/ graph_state_le s2 s1)
+  : exists u : graph_state, forall s : graph_state, s \in C -> graph_state_le s u.
+Proof.
+  destruct NONEMPTY as [s0 IN0]. unshelve eexists.
+  { refine (
+      {|
+        gs_carrier := fun a : A => exists s : graph_state, s \in C /\ gs_carrier s a;
+        gs_nat := _;
+        gs_code := fun x : A => fun y : A => fun z : A => exists s : graph_state, s \in C /\ gs_code s x y z;
+        gs_code_dom := _;
+        gs_code_total := _;
+        gs_code_functional := _;
+        gs_code_inj := _;
+      |}
+    ).
+    - intros n. exists s0. split; [exact IN0 | exact (gs_nat s0 n)].
+    - intros x y z (s & INs & Hcode). pose proof (gs_code_dom s x y z Hcode) as (Hx & Hy & Hz). splits; exists s; split; assumption.
+    - intros x y (sx & INx & Hx) (sy & INy & Hy). pose proof (CHAIN sx sy INx INy) as [LE | LE].
+      + pose proof (gs_code_total sy x y (proj1 LE x Hx) Hy) as [z Hcode]. exists z. exists sy. split; assumption.
+      + pose proof (gs_code_total sx x y Hx (proj1 LE y Hy)) as [z Hcode]. exists z. exists sx. split; assumption.
+    - intros x y z1 z2 (s1 & IN1 & Hcode1) (s2 & IN2 & Hcode2). pose proof (CHAIN s1 s2 IN1 IN2) as [LE | LE].
+      + eapply gs_code_functional; [exact (proj2 LE x y z1 Hcode1) | exact Hcode2].
+      + eapply gs_code_functional; [exact Hcode1 | exact (proj2 LE x y z2 Hcode2)].
+    - intros x1 y1 z1 x2 y2 z2 (s1 & IN1 & Hcode1) (s2 & IN2 & Hcode2) Hz. pose proof (CHAIN s1 s2 IN1 IN2) as [LE | LE].
+      + eapply gs_code_inj; [exact (proj2 LE x1 y1 z1 Hcode1) | exact Hcode2 | exact Hz].
+      + eapply gs_code_inj; [exact Hcode1 | exact (proj2 LE x2 y2 z2 Hcode2) | exact Hz].
+  }
+  intros s INs. split.
+  - intros a Ha. exists s. split; assumption.
+  - intros x y z Hcode. exists s. split; assumption.
+Defined.
+
+Lemma graph_state_maximal_exists
+  : exists m : graph_state, forall t : graph_state, graph_state_le m t -> graph_state_le t m.
+Proof.
+  eapply Zorn's_lemma with (D := graph_state) (PROSET := graph_state_isProset).
+  - econs. exact graph_state_initial.
+  - intros C NONEMPTY CHAIN. eapply graph_state_chain_upperbound; eauto.
+Qed.
+
+Definition graph_state_type (s : graph_state) : Type@{Set_u} :=
+  { a : A | gs_carrier s a }.
+
+Definition graph_state_nat (s : graph_state) (n : nat) : graph_state_type s :=
+  @exist A (gs_carrier s) (nat_embed n) (gs_nat s n).
+
+Lemma graph_state_nat_inj (s : graph_state) (n : nat) (m : nat)
+  (EQ : graph_state_nat s n = graph_state_nat s m)
+  : n = m.
+Proof.
+  eapply nat_embed_inj. injection EQ as EQ_proj. exact EQ_proj.
+Qed.
+
+Definition graph_sum_type (s : graph_state) : Type@{Set_u} :=
+  (graph_state_type s + graph_state_type s)%type.
+
+Definition graph_pair_type (s : graph_state) : Type@{Set_u} :=
+  (graph_sum_type s * graph_sum_type s)%type.
+
+Inductive graph_sum_code (s : graph_state) : graph_sum_type s -> graph_state_type s -> Prop :=
+  | graph_sum_code_l (x : graph_state_type s) (b : graph_state_type s)
+    (CODE : gs_code s (nat_embed O) (proj1_sig x) (proj1_sig b))
+    : graph_sum_code s (inl x) b
+  | graph_sum_code_r (x : graph_state_type s) (b : graph_state_type s)
+    (CODE : gs_code s (nat_embed (S O)) (proj1_sig x) (proj1_sig b))
+    : graph_sum_code s (inr x) b.
+
+Lemma graph_sum_code_total (s : graph_state) (x : graph_sum_type s)
+  : exists b : graph_state_type s, graph_sum_code s x b.
+Proof.
+  destruct x as [x | x].
+  - pose proof (gs_code_total s (nat_embed O) (proj1_sig x) (gs_nat s O) (proj2_sig x)) as [b Hcode].
+    pose proof (gs_code_dom s _ _ _ Hcode) as (_ & _ & Hb). exists (@exist A (gs_carrier s) b Hb). econs. exact Hcode.
+  - pose proof (gs_code_total s (nat_embed (S O)) (proj1_sig x) (gs_nat s (S O)) (proj2_sig x)) as [b Hcode].
+    pose proof (gs_code_dom s _ _ _ Hcode) as (_ & _ & Hb). exists (@exist A (gs_carrier s) b Hb). econs. exact Hcode.
+Qed.
+
+Lemma graph_sum_code_functional (s : graph_state) (x : graph_sum_type s) (b1 : graph_state_type s) (b2 : graph_state_type s)
+  (CODE1 : graph_sum_code s x b1)
+  (CODE2 : graph_sum_code s x b2)
+  : b1 = b2.
+Proof.
+  destruct x as [x | x]; inv CODE1; inv CODE2; eapply Cardinal2.sig_eq_from_proj1; eapply gs_code_functional; eauto.
+Qed.
+
+Lemma graph_sum_code_inj (s : graph_state) (x1 : graph_sum_type s) (x2 : graph_sum_type s) (b1 : graph_state_type s) (b2 : graph_state_type s)
+  (CODE1 : graph_sum_code s x1 b1)
+  (CODE2 : graph_sum_code s x2 b2)
+  (EQ : b1 = b2)
+  : x1 = x2.
+Proof.
+  subst b2.
+  destruct x1 as [x1 | x1], x2 as [x2 | x2]; inv CODE1; inv CODE2.
+  - pose proof (gs_code_inj s _ _ _ _ _ _ CODE CODE0 eq_refl) as [_ EQ_x]. f_equal. eapply Cardinal2.sig_eq_from_proj1. exact EQ_x.
+  - pose proof (gs_code_inj s _ _ _ _ _ _ CODE CODE0 eq_refl) as [EQ_tag _].
+    pose proof (nat_embed_inj O (S O) EQ_tag) as BAD. discriminate BAD.
+  - pose proof (gs_code_inj s _ _ _ _ _ _ CODE CODE0 eq_refl) as [EQ_tag _].
+    pose proof (nat_embed_inj (S O) O EQ_tag) as BAD. discriminate BAD.
+  - pose proof (gs_code_inj s _ _ _ _ _ _ CODE CODE0 eq_refl) as [_ EQ_x]. f_equal. eapply Cardinal2.sig_eq_from_proj1. exact EQ_x.
+Qed.
+
+Inductive graph_pair_code (s : graph_state) : graph_pair_type s -> graph_state_type s -> Prop :=
+  | graph_pair_code_intro (x : graph_sum_type s) (y : graph_sum_type s) (bx : graph_state_type s) (by0 : graph_state_type s) (b : graph_state_type s)
+    (CODE_x : graph_sum_code s x bx)
+    (CODE_y : graph_sum_code s y by0)
+    (CODE : gs_code s (proj1_sig bx) (proj1_sig by0) (proj1_sig b))
+    : graph_pair_code s (x, y) b.
+
+Lemma graph_pair_code_total (s : graph_state) (p : graph_pair_type s)
+  : exists b : graph_state_type s, graph_pair_code s p b.
+Proof.
+  destruct p as [x y]. pose proof (graph_sum_code_total s x) as [bx CODE_x]. pose proof (graph_sum_code_total s y) as [by0 CODE_y].
+  pose proof (gs_code_total s (proj1_sig bx) (proj1_sig by0) (proj2_sig bx) (proj2_sig by0)) as [b CODE].
+  pose proof (gs_code_dom s _ _ _ CODE) as (_ & _ & Hb). exists (@exist A (gs_carrier s) b Hb). econs; eauto.
+Qed.
+
+Lemma graph_pair_code_functional (s : graph_state) (p : graph_pair_type s) (b1 : graph_state_type s) (b2 : graph_state_type s)
+  (CODE1 : graph_pair_code s p b1)
+  (CODE2 : graph_pair_code s p b2)
+  : b1 = b2.
+Proof.
+  inv CODE1. inv CODE2. pose proof (graph_sum_code_functional s _ _ _ CODE_x CODE_x0). subst bx0.
+  pose proof (graph_sum_code_functional s _ _ _ CODE_y CODE_y0). subst by0.
+  eapply Cardinal2.sig_eq_from_proj1. eapply gs_code_functional; eauto.
+Qed.
+
+Lemma graph_pair_code_inj (s : graph_state) (p1 : graph_pair_type s) (p2 : graph_pair_type s) (b1 : graph_state_type s) (b2 : graph_state_type s)
+  (CODE1 : graph_pair_code s p1 b1)
+  (CODE2 : graph_pair_code s p2 b2)
+  (EQ : b1 = b2)
+  : p1 = p2.
+Proof.
+  subst b2. inv CODE1. inv CODE2.
+  pose proof (gs_code_inj s _ _ _ _ _ _ CODE CODE0 eq_refl) as [EQ_bx EQ_by].
+  pose proof (graph_sum_code_inj s _ _ _ _ CODE_x CODE_x0 (Cardinal2.sig_eq_from_proj1 _ _ EQ_bx)) as EQ_x.
+  pose proof (graph_sum_code_inj s _ _ _ _ CODE_y CODE_y0 (Cardinal2.sig_eq_from_proj1 _ _ EQ_by)) as EQ_y.
+  subst. reflexivity.
+Qed.
+
+Definition graph_state_complement_type (s : graph_state) : Type@{Set_u} :=
+  { a : A | ~ gs_carrier s a }.
+
+Inductive graph_extend_repr (s : graph_state) (fresh : graph_state_type s -> graph_state_complement_type s) : A -> graph_sum_type s -> Prop :=
+  | graph_extend_repr_old (b : graph_state_type s)
+    : graph_extend_repr s fresh (proj1_sig b) (inl b)
+  | graph_extend_repr_new (b : graph_state_type s)
+    : graph_extend_repr s fresh (proj1_sig (fresh b)) (inr b).
+
+Definition graph_extend_nonold (s : graph_state) (p : graph_pair_type s) : Prop :=
+  match p with
+  | (inl _, inl _) => False
+  | _ => True
+  end.
+
+Lemma graph_extend_repr_unique (s : graph_state) (fresh : graph_state_type s -> graph_state_complement_type s) (a : A) (x : graph_sum_type s) (y : graph_sum_type s)
+  (fresh_inj : forall b1 : graph_state_type s, forall b2 : graph_state_type s, proj1_sig (fresh b1) = proj1_sig (fresh b2) -> b1 = b2)
+  (REPR_x : graph_extend_repr s fresh a x)
+  (REPR_y : graph_extend_repr s fresh a y)
+  : x = y.
+Proof.
+  inv REPR_x; inv REPR_y.
+  - f_equal. eapply Cardinal2.sig_eq_from_proj1. symmetry. exact H0.
+  - destruct b as [a Ha]. simpl in H0. subst a. contradiction (proj2_sig (fresh b0)).
+  - destruct b0 as [a Ha]. simpl in H0. subst a. contradiction (proj2_sig (fresh b)).
+  - f_equal. eapply fresh_inj. symmetry. exact H0.
+Qed.
+
+Lemma graph_extend_repr_same (s : graph_state) (fresh : graph_state_type s -> graph_state_complement_type s)
+  (a : A) (b : A) (x : graph_sum_type s)
+  (REPR_a : graph_extend_repr s fresh a x)
+  (REPR_b : graph_extend_repr s fresh b x)
+  : a = b.
+Proof.
+  inv REPR_a; inv REPR_b; reflexivity.
+Qed.
+
+Inductive graph_extend_code (s : graph_state) (fresh : graph_state_type s -> graph_state_complement_type s) : A -> A -> A -> Prop :=
+  | graph_extend_code_old (x : A) (y : A) (z : A)
+    (CODE : gs_code s x y z)
+    : graph_extend_code s fresh x y z
+  | graph_extend_code_new (x : A) (y : A) (z : A) (sx : graph_sum_type s) (sy : graph_sum_type s) (b : graph_state_type s)
+    (REPR_x : graph_extend_repr s fresh x sx)
+    (REPR_y : graph_extend_repr s fresh y sy)
+    (NONOLD : graph_extend_nonold s (sx, sy))
+    (CODE : graph_pair_code s (sx, sy) b)
+    (EQ_z : z = proj1_sig (fresh b))
+    : graph_extend_code s fresh x y z.
+
+Lemma graph_extend_repr_of_carrier (s : graph_state) (fresh : graph_state_type s -> graph_state_complement_type s) (a : A)
+  (Ha : exists x : graph_sum_type s, graph_extend_repr s fresh a x)
+  : gs_carrier s a \/ exists b : graph_state_type s, a = proj1_sig (fresh b).
+Proof.
+  destruct Ha as [x Hx]. inv Hx.
+  - left. exact (proj2_sig b).
+  - right. exists b. reflexivity.
+Qed.
+
+Definition graph_state_extend (s : graph_state) (fresh : graph_state_type s -> graph_state_complement_type s)
+  (fresh_inj : forall b1 : graph_state_type s, forall b2 : graph_state_type s, proj1_sig (fresh b1) = proj1_sig (fresh b2) -> b1 = b2)
+  : graph_state.
+Proof.
+  refine (
+    {|
+      gs_carrier := fun a : A => exists x : graph_sum_type s, graph_extend_repr s fresh a x;
+      gs_nat := _;
+      gs_code := graph_extend_code s fresh;
+      gs_code_dom := _;
+      gs_code_total := _;
+      gs_code_functional := _;
+      gs_code_inj := _;
+    |}
+  ).
+  - intros n. exists (inl (graph_state_nat s n)).
+    change (graph_extend_repr s fresh (proj1_sig (graph_state_nat s n)) (inl (graph_state_nat s n))). eapply graph_extend_repr_old.
+  - intros x y z Hcode. inv Hcode.
+    + pose proof (gs_code_dom s x y z CODE) as (Hx & Hy & Hz). splits.
+      * exists (inl (@exist A (gs_carrier s) x Hx)). change (graph_extend_repr s fresh (proj1_sig (@exist A (gs_carrier s) x Hx)) (inl (@exist A (gs_carrier s) x Hx))). eapply graph_extend_repr_old.
+      * exists (inl (@exist A (gs_carrier s) y Hy)). change (graph_extend_repr s fresh (proj1_sig (@exist A (gs_carrier s) y Hy)) (inl (@exist A (gs_carrier s) y Hy))). eapply graph_extend_repr_old.
+      * exists (inl (@exist A (gs_carrier s) z Hz)). change (graph_extend_repr s fresh (proj1_sig (@exist A (gs_carrier s) z Hz)) (inl (@exist A (gs_carrier s) z Hz))). eapply graph_extend_repr_old.
+    + splits; [exists sx | exists sy | exists (inr b)]; eauto using graph_extend_repr_new.
+  - intros x y [sx REPR_x] [sy REPR_y]. destruct sx as [bx | bx], sy as [by0 | by0].
+    + pose proof (gs_code_total s x y) as [z CODE].
+      { inv REPR_x. exact (proj2_sig bx). }
+      { inv REPR_y. exact (proj2_sig by0). }
+      exists z. econs. exact CODE.
+    + pose proof (graph_pair_code_total s (inl bx, inr by0)) as [b CODE]. exists (proj1_sig (fresh b)).
+      eapply graph_extend_code_new with (sx := inl bx) (sy := inr by0) (b := b); eauto.
+      simpl. exact I.
+    + pose proof (graph_pair_code_total s (inr bx, inl by0)) as [b CODE]. exists (proj1_sig (fresh b)).
+      eapply graph_extend_code_new with (sx := inr bx) (sy := inl by0) (b := b); eauto.
+      simpl. exact I.
+    + pose proof (graph_pair_code_total s (inr bx, inr by0)) as [b CODE]. exists (proj1_sig (fresh b)).
+      eapply graph_extend_code_new with (sx := inr bx) (sy := inr by0) (b := b); eauto.
+      simpl. exact I.
+  - intros x y z1 z2 CODE1 CODE2. inv CODE1; inv CODE2.
+    + eapply gs_code_functional; eauto.
+    + pose proof (gs_code_dom s x y z1 CODE) as (Hx & Hy & _).
+      pose proof (graph_extend_repr_unique s fresh x sx (inl (@exist A (gs_carrier s) x Hx)) fresh_inj REPR_x (graph_extend_repr_old s fresh (@exist A (gs_carrier s) x Hx))) as EQ_x.
+      pose proof (graph_extend_repr_unique s fresh y sy (inl (@exist A (gs_carrier s) y Hy)) fresh_inj REPR_y (graph_extend_repr_old s fresh (@exist A (gs_carrier s) y Hy))) as EQ_y.
+      subst sx sy. contradiction.
+    + pose proof (gs_code_dom s x y z2 CODE0) as (Hx & Hy & _).
+      pose proof (graph_extend_repr_unique s fresh x sx (inl (@exist A (gs_carrier s) x Hx)) fresh_inj REPR_x (graph_extend_repr_old s fresh (@exist A (gs_carrier s) x Hx))) as EQ_x.
+      pose proof (graph_extend_repr_unique s fresh y sy (inl (@exist A (gs_carrier s) y Hy)) fresh_inj REPR_y (graph_extend_repr_old s fresh (@exist A (gs_carrier s) y Hy))) as EQ_y.
+      subst sx sy. contradiction.
+    + pose proof (graph_extend_repr_unique s fresh x sx sx0 fresh_inj REPR_x REPR_x0) as EQ_x.
+      pose proof (graph_extend_repr_unique s fresh y sy sy0 fresh_inj REPR_y REPR_y0) as EQ_y.
+      subst sx0 sy0. pose proof (graph_pair_code_functional s _ _ _ CODE CODE0) as EQ_b. subst b0. reflexivity.
+  - intros x1 y1 z1 x2 y2 z2 CODE1 CODE2 EQ_z. inv CODE1; inv CODE2.
+    + eapply gs_code_inj; eauto.
+    + pose proof (gs_code_dom s _ _ _ CODE) as (_ & _ & Hz_old).
+      destruct (fresh b) as [fb Hfb]. simpl in *. subst. contradiction.
+    + pose proof (gs_code_dom s _ _ _ CODE0) as (_ & _ & Hz_old).
+      destruct (fresh b) as [fb Hfb]. simpl in *. subst. contradiction.
+    + pose proof (fresh_inj b b0 EQ_z) as EQ_b. subst b0.
+      pose proof (graph_pair_code_inj s _ _ _ _ CODE CODE0 eq_refl) as EQ_pair. inv EQ_pair.
+      split; eapply graph_extend_repr_same; eauto.
+Defined.
+
+Lemma graph_state_extend_le (s : graph_state) (fresh : graph_state_type s -> graph_state_complement_type s)
+  (fresh_inj : forall b1 : graph_state_type s, forall b2 : graph_state_type s, proj1_sig (fresh b1) = proj1_sig (fresh b2) -> b1 = b2)
+  : graph_state_le s (graph_state_extend s fresh fresh_inj).
+Proof.
+  split.
+  - intros a Ha. exists (inl (@exist A (gs_carrier s) a Ha)).
+    change (graph_extend_repr s fresh (proj1_sig (@exist A (gs_carrier s) a Ha)) (inl (@exist A (gs_carrier s) a Ha))). eapply graph_extend_repr_old.
+  - intros x y z Hcode. econs. exact Hcode.
+Qed.
+
+Lemma graph_state_type_nat_le (s : graph_state)
+  : Cardinality.ofType nat =< Cardinality.ofType (graph_state_type s).
+Proof.
+  eapply Cardinal2.Cardinality_ofType_le_ofType with (f := graph_state_nat s).
+  intros n m EQ. eapply graph_state_nat_inj. exact EQ.
+Qed.
+
+Lemma graph_state_type_prod_le (s : graph_state)
+  : Cardinality.ofType (graph_state_type s * graph_state_type s) =< Cardinality.ofType (graph_state_type s).
+Proof.
+  assert (Hchoice : forall p : graph_state_type s * graph_state_type s, exists b : graph_state_type s, gs_code s (proj1_sig (Datatypes.fst p)) (proj1_sig (Datatypes.snd p)) (proj1_sig b)).
+  { intros [x y]. pose proof (gs_code_total s (proj1_sig x) (proj1_sig y) (proj2_sig x) (proj2_sig y)) as [z CODE].
+    pose proof (gs_code_dom s _ _ _ CODE) as (_ & _ & Hz). exists (@exist A (gs_carrier s) z Hz). exact CODE.
+  }
+  pose proof (Axiom_of_Choice (graph_state_type s * graph_state_type s) (fun _ : graph_state_type s * graph_state_type s => graph_state_type s) (fun p : graph_state_type s * graph_state_type s => fun b : graph_state_type s => gs_code s (proj1_sig (Datatypes.fst p)) (proj1_sig (Datatypes.snd p)) (proj1_sig b)) Hchoice) as [code CODE].
+  eapply Cardinal2.Cardinality_ofType_le_ofType with (f := code).
+  intros [x1 y1] [x2 y2] EQ. change (code (x1, y1) = code (x2, y2)) in EQ.
+  assert (EQ_proj : proj1_sig (code (x1, y1)) = proj1_sig (code (x2, y2))) by now rewrite EQ.
+  pose proof (gs_code_inj s _ _ _ _ _ _ (CODE (x1, y1)) (CODE (x2, y2)) EQ_proj) as [EQ_x EQ_y].
+  f_equal; eapply Cardinal2.sig_eq_from_proj1; assumption.
+Qed.
+
+Definition graph_cover_sum_type (s : graph_state) : Type@{Set_u} :=
+  (graph_state_type s + graph_state_complement_type s)%type.
+
+Definition graph_sum_proj (s : graph_state) (x : graph_cover_sum_type s) : A :=
+  match x with
+  | inl b => proj1_sig b
+  | inr c => proj1_sig c
+  end.
+
+Lemma graph_state_cover_le_sum (s : graph_state)
+  : Cardinality.ofType A =< Cardinality.ofType (graph_cover_sum_type s).
+Proof.
+  assert (Hchoice : forall a : A, exists x : graph_cover_sum_type s, graph_sum_proj s x = a).
+  { intros a. pose proof (classic (gs_carrier s a)) as [Ha | Ha].
+    - exists (inl (@exist A (gs_carrier s) a Ha)). reflexivity.
+    - exists (inr (@exist A (fun x : A => ~ gs_carrier s x) a Ha)). reflexivity.
+  }
+  pose proof (Axiom_of_Choice A (fun _ : A => graph_cover_sum_type s) (fun a : A => fun x : graph_cover_sum_type s => graph_sum_proj s x = a) Hchoice) as [pick PICK].
+  eapply Cardinal2.Cardinality_ofType_le_ofType with (f := pick).
+  intros a1 a2 EQ. change (pick a1 = pick a2) in EQ. rewrite <- (PICK a1). rewrite <- (PICK a2). now rewrite EQ.
+Qed.
+
+Lemma graph_state_complement_le_carrier (m : graph_state)
+  (MAX : forall t : graph_state, graph_state_le m t -> graph_state_le t m)
+  : Cardinality.ofType (graph_state_complement_type m) =< Cardinality.ofType (graph_state_type m).
+Proof.
+  pose proof (Cardinal1.Cardinality_le_total (Cardinality.ofType (graph_state_type m)) (Cardinality.ofType (graph_state_complement_type m))) as [LE | LE].
+  - destruct LE as [fresh fresh_cong fresh_inj].
+    assert (fresh_inj_proj : forall b1 : graph_state_type m, forall b2 : graph_state_type m, proj1_sig (fresh b1) = proj1_sig (fresh b2) -> b1 = b2).
+    { intros b1 b2 EQ. eapply fresh_inj. change (fresh b1 = fresh b2). eapply Cardinal2.sig_eq_from_proj1. exact EQ. }
+    pose proof (MAX (graph_state_extend m fresh fresh_inj_proj) (graph_state_extend_le m fresh fresh_inj_proj)) as BACK.
+    pose (b0 := graph_state_nat m O).
+    pose proof (proj1 BACK (proj1_sig (fresh b0))) as IN_BACK.
+    assert (IN_EXT : gs_carrier (graph_state_extend m fresh fresh_inj_proj) (proj1_sig (fresh b0))).
+    { exists (inr b0). econs. }
+    specialize (IN_BACK IN_EXT). exact (False_rect _ (proj2_sig (fresh b0) IN_BACK)).
+  - exact LE.
+Qed.
+
+End GRAPH_SQUARE_ABSORPTION.
+
+Theorem Cardinality_ofType_prod_self_le_of_nat_le (A : Type@{Set_u})
+  (NAT_LE : Cardinality.ofType nat =< Cardinality.ofType A)
+  : Cardinality.ofType (A * A) =< Cardinality.ofType A.
+Proof.
+  destruct NAT_LE as [nat_emb nat_emb_cong nat_emb_inj].
+  assert (nat_emb_inj_raw : forall n : nat, forall m : nat, nat_emb n = nat_emb m -> n = m).
+  { intros n m EQ. eapply nat_emb_inj. change (nat_emb n = nat_emb m). exact EQ. }
+  pose proof (@graph_state_maximal_exists A nat_emb nat_emb_inj_raw) as [m MAX].
+  pose proof (@graph_state_type_nat_le A nat_emb nat_emb_inj_raw m) as NAT_LE_B.
+  pose proof (@graph_state_type_prod_le A nat_emb m) as PROD_B_LE_B.
+  pose proof (@graph_state_complement_le_carrier A nat_emb nat_emb_inj_raw m MAX) as COMP_LE_B.
+  assert (B_LE_A : Cardinality.ofType (graph_state_type A nat_emb m) =< Cardinality.ofType A).
+  { eapply Cardinal2.Cardinality_ofType_sig_le. }
+  assert (A_LE_B : Cardinality.ofType A =< Cardinality.ofType (graph_state_type A nat_emb m)).
+  { transitivity (Cardinality.ofType (graph_cover_sum_type A nat_emb m)).
+    - eapply graph_state_cover_le_sum.
+    - transitivity (Cardinality.mul (Cardinality.ofType bool) (Cardinality.ofType (graph_state_type A nat_emb m))).
+      + eapply Cardinal2.Cardinality_ofType_sum_le.
+        * reflexivity.
+        * exact COMP_LE_B.
+      + transitivity (Cardinality.ofType (graph_state_type A nat_emb m * graph_state_type A nat_emb m)).
+        * pose proof (Cardinal2.Cardinality_ofType_prod_eq bool (graph_state_type A nat_emb m)) as PROD_EQ. rewrite <- PROD_EQ.
+          eapply Cardinal2.Cardinality_ofType_prod_le.
+          { eapply Cardinality_ofType_bool_le_of_nat_le. exact NAT_LE_B. }
+          { reflexivity. }
+        * exact PROD_B_LE_B.
+  }
+  transitivity (Cardinality.ofType (graph_state_type A nat_emb m * graph_state_type A nat_emb m)).
+  - eapply Cardinal2.Cardinality_ofType_prod_le; exact A_LE_B.
+  - transitivity (Cardinality.ofType (graph_state_type A nat_emb m)); [exact PROD_B_LE_B | exact B_LE_A].
+Qed.
+
+Theorem Cardinality_ofType_rose_lt_of_lt_uncountable (A : Type@{Set_u}) (kappa : Cardinality.t)
+  (LT : Cardinality.ofType A ≨ kappa)
+  (UNCOUNTABLE : ~ kappa =< Cardinality.ofType nat)
+  : Cardinality.ofType (B.rose A) ≨ kappa.
+Proof.
+  eapply Cardinality_ofType_rose_lt_of_lt_uncountable_square_le; eauto.
+  intros B NAT_LE. eapply Cardinality_ofType_prod_self_le_of_nat_le. exact NAT_LE.
+Qed.
+
+End CARDINALITY.
+
+End Cardinal3.
+
+Module Inaccessible.
+
+Section CLASSICAL.
+
+#[local] Existing Instance Ord_isProset.
+
+Record inaccessible (X : Type@{Set_u}) (base : Ord.t) (next : Ord.t -> Ord.t) (k : Ord.t) : Prop :=
+  mk_inaccessible
+  { inaccessible_base : base <ᵣ k
+  ; inaccessible_next : forall alpha : Ord.t, alpha <ᵣ k -> next alpha <ᵣ k
+  ; inaccessible_join : forall os : X -> Ord.t, (forall x : X, os x <ᵣ k) -> Ord.sup X os <ᵣ k
+  ; inaccessible_union : forall alpha : Ord.t, forall beta : Ord.t, alpha <ᵣ k -> beta <ᵣ k -> Ord_join alpha beta <ᵣ k
+  }.
+
+Record ginaccessible (X : Type@{Set_u}) (base : Ord.t) (next : Ord.t -> Ord.t) (k : Ord.t) : Prop :=
+  mk_ginaccessible
+  { ginaccessible_base : base <ᵣ k
+  ; ginaccessible_next : forall alpha : Ord.t, alpha <ᵣ k -> next alpha <ᵣ k
+  ; ginaccessible_join : forall P : X -> Prop, forall os : @sig X P -> Ord.t, (forall x : @sig X P, os x <ᵣ k) -> Ord.sup (@sig X P) os <ᵣ k
+  ; ginaccessible_union : forall alpha : Ord.t, forall beta : Ord.t, alpha <ᵣ k -> beta <ᵣ k -> Ord_join alpha beta <ᵣ k
+  }.
+
+Context `{Axms : ClassicalAxioms (b_AC := true) (b_fun_ext := true) (b_prop_ext := true)}.
+
+Lemma inaccessible_mon (X0 : Type@{Set_u}) (X1 : Type@{Set_u}) (base0 : Ord.t) (base1 : Ord.t) (next0 : Ord.t -> Ord.t) (next1 : Ord.t -> Ord.t) (k : Ord.t)
+  (H_surj : exists f : X1 -> X0, forall x0 : X0, exists x1 : X1, f x1 = x0)
+  (H_base : base0 <ᵣ k)
+  (H_next : forall alpha : Ord.t, alpha <ᵣ k -> next0 alpha ≦ᵣ next1 alpha)
+  (H_inaccessible : inaccessible X1 base1 next1 k)
+  : inaccessible X0 base0 next0 k.
+Proof.
+  destruct H_surj as [f H_surj]. econs.
+  - exact H_base.
+  - intros alpha H_rLt. eapply rLe_rLt_rLt.
+    + eapply H_next. exact H_rLt.
+    + eapply H_inaccessible. exact H_rLt.
+  - intros os H_rLt. eapply rLe_rLt_rLt with (y := Ord.sup X1 (fun x1 : X1 => os (f x1))).
+    + eapply Ord_sup_rLe_intro. intros x0. pose proof (H_surj x0) as [x1 H_eq]. subst x0.
+      change ((fun x1 : X1 => os (f x1)) x1 ≦ᵣ Ord.sup X1 (fun x2 : X1 => os (f x2))). eapply Ord_rLe_sup_intro.
+    + eapply H_inaccessible. intros x1. eapply H_rLt.
+  - intros alpha beta H_rLt0 H_rLt1. eapply H_inaccessible; assumption.
+Qed.
+
+Lemma ginaccessible_inaccessible (X : Type@{Set_u}) (base : Ord.t) (next : Ord.t -> Ord.t) (k : Ord.t)
+  (H_inaccessible : ginaccessible X base next k)
+  : inaccessible X base next k.
+Proof.
+  econs.
+  - eapply H_inaccessible.
+  - eapply H_inaccessible.
+  - intros os H_rLt. eapply rLe_rLt_rLt with (y := Ord.sup (@sig X (fun _ : X => True)) (fun x : @sig X (fun _ : X => True) => os (proj1_sig x))).
+    + eapply Ord_sup_rLe_intro. intros x.
+      change ((fun x : @sig X (fun _ : X => True) => os (proj1_sig x)) (@exist X (fun _ : X => True) x I) ≦ᵣ Ord.sup (@sig X (fun _ : X => True)) (fun x0 : @sig X (fun _ : X => True) => os (proj1_sig x0))).
+      eapply Ord_rLe_sup_intro.
+    + eapply H_inaccessible. intros x. eapply H_rLt.
+  - eapply H_inaccessible.
+Qed.
+
+Inductive tree {X : Type@{Set_u}} : Type@{Set_u} :=
+  | tree_O : @tree X
+  | tree_S : @tree X -> @tree X
+  | tree_join : (X -> @tree X) -> @tree X
+  | tree_union : @tree X -> @tree X -> @tree X.
+
+#[global] Arguments tree : clear implicits.
+
+Definition tree_lt {X : Type@{Set_u}} (tr0 : tree X) (tr1 : tree X) : Prop :=
+  match tr1 with
+  | tree_O => False
+  | tree_S tr => tr0 = tr
+  | tree_join trs => exists x : X, tr0 = trs x
+  | tree_union trl trr => tr0 = trl \/ tr0 = trr
+  end.
+
+Lemma tree_lt_well_founded (X : Type@{Set_u})
+  : well_founded (@tree_lt X).
+Proof.
+  ii. induction a as [ | tr IH | trs IH | tr0 IH0 tr1 IH1].
+  - econs. intros y H_rLt. contradiction.
+  - econs. intros y H_rLt. simpl in H_rLt. subst y. exact IH.
+  - econs. intros y H_rLt. simpl in H_rLt. destruct H_rLt as [x ->]. exact (IH x).
+  - econs. intros y H_rLt. simpl in H_rLt. destruct H_rLt as [-> | ->]; assumption.
+Qed.
+
+Definition tree_top (X : Type@{Set_u}) : Ord.t :=
+  @fromWfSet (tree X) (@tree_lt X) (tree_lt_well_founded X).
+
+Lemma tree_O_rEq (X : Type@{Set_u})
+  : @fromWf (tree X) (@tree_lt X) (tree_lt_well_founded X) tree_O =ᵣ Ord.zer.
+Proof.
+  rewrite rEq_iff. split.
+  - eapply fromWf_isSupremum. intros y H_rLt. contradiction H_rLt.
+  - eapply Ord_zer_rLe.
+Qed.
+
+Lemma tree_S_rEq (X : Type@{Set_u}) (tr : tree X)
+  : @fromWf (tree X) (@tree_lt X) (tree_lt_well_founded X) (tree_S tr) =ᵣ Ord.suc (@fromWf (tree X) (@tree_lt X) (tree_lt_well_founded X) tr).
+Proof.
+  rewrite rEq_iff. split.
+  - eapply fromWf_isSupremum. intros y H_rLt. simpl in H_rLt. subst y. unfold Ord.suc. eapply rLt_succ_intro.
+  - unfold Ord.suc. rewrite succ_rLe_iff. eapply member_implies_rLt. rewrite fromWf_unfold.
+    exists tr. split; [reflexivity | reflexivity].
+Qed.
+
+Lemma tree_join_rEq (X : Type@{Set_u}) (trs : X -> tree X)
+  : @fromWf (tree X) (@tree_lt X) (tree_lt_well_founded X) (tree_join trs) =ᵣ mkNode X (fun x : X => @fromWf (tree X) (@tree_lt X) (tree_lt_well_founded X) (trs x)).
+Proof.
+  rewrite rEq_iff. split.
+  - eapply fromWf_isSupremum. intros y H_rLt. simpl in H_rLt. destruct H_rLt as [x ->].
+    eapply member_implies_rLt. exists x. reflexivity.
+  - econs. intros x. eapply member_implies_rLt. rewrite fromWf_unfold.
+    exists (trs x). split; [now exists x | reflexivity].
+Qed.
+
+Lemma tree_union_le (X : Type@{Set_u}) (tr0 : tree X) (tr1 : tree X)
+  : @fromWf (tree X) (@tree_lt X) (tree_lt_well_founded X) (tree_union tr0 tr1) ≦ᵣ Ord.suc (Ord_join (@fromWf (tree X) (@tree_lt X) (tree_lt_well_founded X) tr0) (@fromWf (tree X) (@tree_lt X) (tree_lt_well_founded X) tr1)).
+Proof.
+  eapply fromWf_isSupremum. intros y H_rLt. simpl in H_rLt. unfold Ord.suc. rewrite rLt_succ_iff. destruct H_rLt as [-> | ->].
+  - eapply Ord_join_l.
+  - eapply Ord_join_r.
+Qed.
+
+Lemma tree_union_le_rev (X : Type@{Set_u}) (tr0 : tree X) (tr1 : tree X)
+  : Ord_join (@fromWf (tree X) (@tree_lt X) (tree_lt_well_founded X) tr0) (@fromWf (tree X) (@tree_lt X) (tree_lt_well_founded X) tr1) ≦ᵣ @fromWf (tree X) (@tree_lt X) (tree_lt_well_founded X) (tree_union tr0 tr1).
+Proof.
+  eapply Ord_join_spec; eapply rLt_implies_rLe; eapply member_implies_rLt; rewrite fromWf_unfold.
+  - exists tr0. now split; [left | reflexivity].
+  - exists tr1. now split; [right | reflexivity].
+Qed.
+
+Lemma tree_top_O (X : Type@{Set_u})
+  : Ord.zer <ᵣ tree_top X.
+Proof.
+  eapply rLe_rLt_rLt with (y := @fromWf (tree X) (@tree_lt X) (tree_lt_well_founded X) tree_O).
+  - exact (proj2 (tree_O_rEq X)).
+  - eapply member_implies_rLt. exists tree_O. reflexivity.
+Qed.
+
+Lemma tree_top_S (X : Type@{Set_u}) (alpha : Ord.t)
+  (H_rLt : alpha <ᵣ tree_top X)
+  : Ord.suc alpha <ᵣ tree_top X.
+Proof.
+  destruct H_rLt as [[tr H_rLe]]. eapply rLe_rLt_rLt with (y := @fromWf (tree X) (@tree_lt X) (tree_lt_well_founded X) (tree_S tr)).
+  - transitivity (Ord.suc (@fromWf (tree X) (@tree_lt X) (tree_lt_well_founded X) tr)).
+    + eapply Ord_suc_rLe. exact H_rLe.
+    + exact (proj2 (tree_S_rEq X tr)).
+  - eapply member_implies_rLt. exists (tree_S tr). reflexivity.
+Qed.
+
+Lemma tree_top_union (X : Type@{Set_u}) (alpha : Ord.t) (beta : Ord.t)
+  (H_rLt0 : alpha <ᵣ tree_top X)
+  (H_rLt1 : beta <ᵣ tree_top X)
+  : Ord_join alpha beta <ᵣ tree_top X.
+Proof.
+  destruct H_rLt0 as [[tr0 H_rLe0]], H_rLt1 as [[tr1 H_rLe1]].
+  eapply rLe_rLt_rLt with (y := @fromWf (tree X) (@tree_lt X) (tree_lt_well_founded X) (tree_union tr0 tr1)).
+  - transitivity (Ord_join (@fromWf (tree X) (@tree_lt X) (tree_lt_well_founded X) tr0) (@fromWf (tree X) (@tree_lt X) (tree_lt_well_founded X) tr1)).
+    + eapply Ord_join_spec.
+      * transitivity (@fromWf (tree X) (@tree_lt X) (tree_lt_well_founded X) tr0); [exact H_rLe0 | eapply Ord_join_l].
+      * transitivity (@fromWf (tree X) (@tree_lt X) (tree_lt_well_founded X) tr1); [exact H_rLe1 | eapply Ord_join_r].
+    + eapply tree_union_le_rev.
+  - eapply member_implies_rLt. exists (tree_union tr0 tr1). reflexivity.
+Qed.
+
+Lemma tree_top_join (X : Type@{Set_u}) (os : X -> Ord.t)
+  (H_rLt : forall x : X, os x <ᵣ tree_top X)
+  : Ord.sup X os <ᵣ tree_top X.
+Proof.
+  exploit (Axiom_of_Choice X (fun _ : X => tree X) (fun x : X => fun tr : tree X => os x ≦ᵣ @fromWf (tree X) (@tree_lt X) (tree_lt_well_founded X) tr)).
+  { intros x. pose proof (H_rLt x) as [[tr H_rLe]]. exists tr. exact H_rLe. }
+  intros [f H_f]. eapply rLe_rLt_rLt with (y := @fromWf (tree X) (@tree_lt X) (tree_lt_well_founded X) (tree_join f)).
+  - eapply Ord_sup_rLe_intro. intros x. transitivity (@fromWf (tree X) (@tree_lt X) (tree_lt_well_founded X) (f x)).
+    + eapply H_f.
+    + eapply rLt_implies_rLe. eapply member_implies_rLt. rewrite fromWf_unfold.
+      exists (f x). split; [now exists x | reflexivity].
+  - eapply member_implies_rLt. exists (tree_join f). reflexivity.
+Qed.
+
+Lemma tree_top_S_inaccessible (X : Type@{Set_u})
+  : inaccessible X Ord.zer Ord.suc (tree_top X).
+Proof.
+  econs.
+  - eapply tree_top_O.
+  - eapply tree_top_S.
+  - eapply tree_top_join.
+  - eapply tree_top_union.
+Qed.
+
+Lemma tree_top_orec (X : Type@{Set_u}) (base0 : Ord.t) (next : Ord.t -> Ord.t) (base1 : Ord.t)
+  (H_next_le : forall alpha : Ord.t, alpha ≦ᵣ next alpha)
+  (H_next_mon : forall alpha : Ord.t, forall beta : Ord.t, alpha ≦ᵣ beta -> next alpha ≦ᵣ next beta)
+  (H_inaccessible : inaccessible X base0 next (tree_top X))
+  (H_base1 : base1 <ᵣ tree_top X)
+  : forall alpha : Ord.t, alpha <ᵣ tree_top X -> Ord.orec base1 next alpha <ᵣ tree_top X.
+Proof.
+  intros alpha H_rLt.
+  enough (H_recs : forall tr : tree X, Ord.orec base1 next (@fromWf (tree X) (@tree_lt X) (tree_lt_well_founded X) tr) <ᵣ tree_top X).
+  { destruct H_rLt as [[tr H_rLe]]. eapply rLe_rLt_rLt; [eapply Ord_orec_rLe; eauto; exact H_rLe | eapply H_recs]. }
+  intros tr. induction tr as [ | tr IH | trs IH | tr0 IH0 tr1 IH1].
+  - eapply rLe_rLt_rLt with (y := base1).
+    + pose proof (Ord_orec_rEq_r base1 next (@fromWf (tree X) (@tree_lt X) (tree_lt_well_founded X) tree_O) Ord.zer H_next_le H_next_mon (tree_O_rEq X)) as H_eq.
+      pose proof (Ord_orec_zer base1 next) as H_eq0. transitivity (Ord.orec base1 next Ord.zer).
+      * eapply H_eq.
+      * exact (proj1 H_eq0).
+    + exact H_base1.
+  - eapply rLe_rLt_rLt with (y := next (Ord.orec base1 next (@fromWf (tree X) (@tree_lt X) (tree_lt_well_founded X) tr))).
+    + pose proof (Ord_orec_rEq_r base1 next (@fromWf (tree X) (@tree_lt X) (tree_lt_well_founded X) (tree_S tr)) (Ord.suc (@fromWf (tree X) (@tree_lt X) (tree_lt_well_founded X) tr)) H_next_le H_next_mon (tree_S_rEq X tr)) as H_eq.
+      transitivity (Ord.orec base1 next (Ord.suc (@fromWf (tree X) (@tree_lt X) (tree_lt_well_founded X) tr))).
+      * eapply H_eq.
+      * exact (proj1 (Ord_orec_suc base1 next H_next_le H_next_mon (@fromWf (tree X) (@tree_lt X) (tree_lt_well_founded X) tr))).
+    + eapply H_inaccessible. exact IH.
+  - eapply rLe_rLt_rLt with (y := Ord_join base1 (Ord.sup X (fun x : X => next (Ord.orec base1 next (@fromWf (tree X) (@tree_lt X) (tree_lt_well_founded X) (trs x)))))).
+    + transitivity (Ord.orec base1 next (mkNode X (fun x : X => @fromWf (tree X) (@tree_lt X) (tree_lt_well_founded X) (trs x)))).
+      * eapply Ord_orec_rEq_r with (base := base1) (next := next) (alpha := @fromWf (tree X) (@tree_lt X) (tree_lt_well_founded X) (tree_join trs)) (beta := mkNode X (fun x : X => @fromWf (tree X) (@tree_lt X) (tree_lt_well_founded X) (trs x))); [exact H_next_le | exact H_next_mon | exact (tree_join_rEq X trs)].
+      * rewrite Ord_orec_unfold. reflexivity.
+    + eapply H_inaccessible.
+      * exact H_base1.
+      * eapply H_inaccessible. intros x. eapply H_inaccessible. exact (IH x).
+  - eapply rLe_rLt_rLt with (y := Ord.orec base1 next (Ord.suc (Ord_join (@fromWf (tree X) (@tree_lt X) (tree_lt_well_founded X) tr0) (@fromWf (tree X) (@tree_lt X) (tree_lt_well_founded X) tr1)))).
+    + eapply Ord_orec_rLe; eauto. eapply tree_union_le.
+    + eapply rLe_rLt_rLt with (y := next (Ord.orec base1 next (Ord_join (@fromWf (tree X) (@tree_lt X) (tree_lt_well_founded X) tr0) (@fromWf (tree X) (@tree_lt X) (tree_lt_well_founded X) tr1)))).
+      * exact (proj1 (Ord_orec_suc base1 next H_next_le H_next_mon (Ord_join (@fromWf (tree X) (@tree_lt X) (tree_lt_well_founded X) tr0) (@fromWf (tree X) (@tree_lt X) (tree_lt_well_founded X) tr1)))).
+      * eapply H_inaccessible. eapply rLe_rLt_rLt with (y := Ord_join (Ord.orec base1 next (@fromWf (tree X) (@tree_lt X) (tree_lt_well_founded X) tr0)) (Ord.orec base1 next (@fromWf (tree X) (@tree_lt X) (tree_lt_well_founded X) tr1))).
+        { exact (proj1 (Ord_orec_join base1 next (@fromWf (tree X) (@tree_lt X) (tree_lt_well_founded X) tr0) (@fromWf (tree X) (@tree_lt X) (tree_lt_well_founded X) tr1) H_next_le H_next_mon)). }
+        { eapply H_inaccessible; assumption. }
+Qed.
+
+Lemma tree_top_rec_inaccessible (X : Type@{Set_u}) (base0 : Ord.t) (next : Ord.t -> Ord.t) (base1 : Ord.t)
+  (H_next_le : forall alpha : Ord.t, alpha ≦ᵣ next alpha)
+  (H_next_mon : forall alpha : Ord.t, forall beta : Ord.t, alpha ≦ᵣ beta -> next alpha ≦ᵣ next beta)
+  (H_inaccessible : inaccessible X base0 next (tree_top X))
+  (H_base1 : base1 <ᵣ tree_top X)
+  : inaccessible X base0 (Ord.orec base1 next) (tree_top X).
+Proof.
+  econs.
+  - eapply H_inaccessible.
+  - eapply tree_top_orec; eauto.
+  - eapply H_inaccessible.
+  - eapply H_inaccessible.
+Qed.
+
+Lemma tree_top_add_inaccessible (X : Type@{Set_u}) (alpha : Ord.t)
+  (H_rLt : alpha <ᵣ tree_top X)
+  : inaccessible X Ord.zer (Ord.add alpha) (tree_top X).
+Proof.
+  unfold Ord.add. eapply tree_top_rec_inaccessible; eauto.
+  - intros x. eapply Ord_rLe_suc.
+  - intros x y H_rLe. eapply Ord_suc_rLe. exact H_rLe.
+  - eapply tree_top_S_inaccessible.
+Qed.
+
+Lemma tree_top_add (X : Type@{Set_u}) (alpha : Ord.t) (beta : Ord.t)
+  (H_rLt0 : alpha <ᵣ tree_top X)
+  (H_rLt1 : beta <ᵣ tree_top X)
+  : Ord.add alpha beta <ᵣ tree_top X.
+Proof.
+  eapply tree_top_add_inaccessible; eauto.
+Qed.
+
+Lemma tree_top_flip_add_inaccessible (X : Type@{Set_u}) (alpha : Ord.t)
+  (H_rLt : alpha <ᵣ tree_top X)
+  : inaccessible X Ord.zer (fun x : Ord.t => Ord.add x alpha) (tree_top X).
+Proof.
+  econs.
+  - eapply tree_top_O.
+  - intros x LT_x. eapply tree_top_add; eauto.
+  - eapply tree_top_join.
+  - eapply tree_top_union.
+Qed.
+
+Lemma tree_top_mul_inaccessible (X : Type@{Set_u}) (alpha : Ord.t)
+  (H_rLt : alpha <ᵣ tree_top X)
+  : inaccessible X Ord.zer (Ord.mul alpha) (tree_top X).
+Proof.
+  unfold Ord.mul. eapply tree_top_rec_inaccessible; eauto.
+  - intros x. eapply Ord_add_base_l.
+  - intros x y H_rLe. eapply Ord_add_rLe_l. exact H_rLe.
+  - eapply tree_top_flip_add_inaccessible. exact H_rLt.
+  - eapply tree_top_O.
+Qed.
+
+Lemma tree_top_mul (X : Type@{Set_u}) (alpha : Ord.t) (beta : Ord.t)
+  (H_rLt0 : alpha <ᵣ tree_top X)
+  (H_rLt1 : beta <ᵣ tree_top X)
+  : Ord.mul alpha beta <ᵣ tree_top X.
+Proof.
+  eapply tree_top_mul_inaccessible; eauto.
+Qed.
+
+Lemma tree_top_flip_mul_inaccessible (X : Type@{Set_u}) (alpha : Ord.t)
+  (H_rLt : alpha <ᵣ tree_top X)
+  : inaccessible X Ord.zer (fun x : Ord.t => Ord.mul x alpha) (tree_top X).
+Proof.
+  econs.
+  - eapply tree_top_O.
+  - intros x LT_x. eapply tree_top_mul; eauto.
+  - eapply tree_top_join.
+  - eapply tree_top_union.
+Qed.
+
+Lemma tree_top_exp_inaccessible (X : Type@{Set_u}) (alpha : Ord.t)
+  (H_pos : Ord.zer <ᵣ alpha)
+  (H_rLt : alpha <ᵣ tree_top X)
+  : inaccessible X Ord.zer (Ord.exp alpha) (tree_top X).
+Proof.
+  unfold Ord.exp. eapply tree_top_rec_inaccessible; eauto.
+  - intros x. eapply Ord_mul_base_l. exact H_pos.
+  - intros x y H_rLe. eapply Ord_mul_rLe_l. exact H_rLe.
+  - eapply tree_top_flip_mul_inaccessible. exact H_rLt.
+  - unfold Ord.one. eapply tree_top_S. eapply tree_top_O.
+Qed.
+
+Lemma tree_top_exp (X : Type@{Set_u}) (alpha : Ord.t) (beta : Ord.t)
+  (H_rLt0 : alpha <ᵣ tree_top X)
+  (H_rLt1 : beta <ᵣ tree_top X)
+  : Ord.exp alpha beta <ᵣ tree_top X.
+Proof.
+  eapply rLe_rLt_rLt with (y := Ord.exp (Ord.suc alpha) beta).
+  - eapply Ord_exp_rLe_l. eapply Ord_rLe_suc.
+  - eapply tree_top_exp_inaccessible.
+    + eapply rLe_rLt_rLt with (y := alpha); [eapply Ord_zer_rLe | unfold Ord.suc; eapply rLt_succ_intro].
+    + eapply tree_top_S. exact H_rLt0.
+    + exact H_rLt1.
+Qed.
+
+Lemma tree_top_flip_exp_inaccessible (X : Type@{Set_u}) (alpha : Ord.t)
+  (H_rLt : alpha <ᵣ tree_top X)
+  : inaccessible X Ord.zer (fun x : Ord.t => Ord.exp x alpha) (tree_top X).
+Proof.
+  econs.
+  - eapply tree_top_O.
+  - intros x LT_x. eapply tree_top_exp; eauto.
+  - eapply tree_top_join.
+  - eapply tree_top_union.
+Qed.
+
+Inductive gtree {X : Type@{Set_u}} : Type@{Set_u} :=
+  | gtree_O : @gtree X
+  | gtree_S : @gtree X -> @gtree X
+  | gtree_join : forall P : X -> Prop, (@sig X P -> @gtree X) -> @gtree X
+  | gtree_union : @gtree X -> @gtree X -> @gtree X.
+
+#[global] Arguments gtree : clear implicits.
+
+Definition gtree_lt {X : Type@{Set_u}} (tr0 : gtree X) (tr1 : gtree X) : Prop :=
+  match tr1 with
+  | gtree_O => False
+  | gtree_S tr => tr0 = tr
+  | gtree_join P trs => exists x : @sig X P, tr0 = trs x
+  | gtree_union trl trr => tr0 = trl \/ tr0 = trr
+  end.
+
+Lemma gtree_lt_well_founded (X : Type@{Set_u})
+  : well_founded (@gtree_lt X).
+Proof.
+  ii. induction a as [ | tr IH | P trs IH | tr0 IH0 tr1 IH1].
+  - econs. intros y H_rLt. contradiction.
+  - econs. intros y H_rLt. simpl in H_rLt. subst y. exact IH.
+  - econs. intros y H_rLt. simpl in H_rLt. destruct H_rLt as [x ->]. exact (IH x).
+  - econs. intros y H_rLt. simpl in H_rLt. destruct H_rLt as [-> | ->]; assumption.
+Qed.
+
+Definition gtree_top (X : Type@{Set_u}) : Ord.t :=
+  @fromWfSet (gtree X) (@gtree_lt X) (gtree_lt_well_founded X).
+
+Lemma gtree_O_rEq (X : Type@{Set_u})
+  : @fromWf (gtree X) (@gtree_lt X) (gtree_lt_well_founded X) gtree_O =ᵣ Ord.zer.
+Proof.
+  rewrite rEq_iff. split.
+  - eapply fromWf_isSupremum. intros y H_rLt. contradiction H_rLt.
+  - eapply Ord_zer_rLe.
+Qed.
+
+Lemma gtree_S_rEq (X : Type@{Set_u}) (tr : gtree X)
+  : @fromWf (gtree X) (@gtree_lt X) (gtree_lt_well_founded X) (gtree_S tr) =ᵣ Ord.suc (@fromWf (gtree X) (@gtree_lt X) (gtree_lt_well_founded X) tr).
+Proof.
+  rewrite rEq_iff. split.
+  - eapply fromWf_isSupremum. intros y H_rLt. simpl in H_rLt. subst y. unfold Ord.suc. eapply rLt_succ_intro.
+  - unfold Ord.suc. rewrite succ_rLe_iff. eapply member_implies_rLt. rewrite fromWf_unfold.
+    exists tr. split; [reflexivity | reflexivity].
+Qed.
+
+Lemma gtree_join_rEq (X : Type@{Set_u}) (P : X -> Prop) (trs : @sig X P -> gtree X)
+  : @fromWf (gtree X) (@gtree_lt X) (gtree_lt_well_founded X) (gtree_join P trs) =ᵣ mkNode (@sig X P) (fun x : @sig X P => @fromWf (gtree X) (@gtree_lt X) (gtree_lt_well_founded X) (trs x)).
+Proof.
+  rewrite rEq_iff. split.
+  - eapply fromWf_isSupremum. intros y H_rLt. simpl in H_rLt. destruct H_rLt as [x ->].
+    eapply member_implies_rLt. exists x. reflexivity.
+  - econs. intros x. eapply member_implies_rLt. rewrite fromWf_unfold.
+    exists (trs x). split; [now exists x | reflexivity].
+Qed.
+
+Lemma gtree_union_le (X : Type@{Set_u}) (tr0 : gtree X) (tr1 : gtree X)
+  : @fromWf (gtree X) (@gtree_lt X) (gtree_lt_well_founded X) (gtree_union tr0 tr1) ≦ᵣ Ord.suc (Ord_join (@fromWf (gtree X) (@gtree_lt X) (gtree_lt_well_founded X) tr0) (@fromWf (gtree X) (@gtree_lt X) (gtree_lt_well_founded X) tr1)).
+Proof.
+  eapply fromWf_isSupremum. intros y H_rLt. simpl in H_rLt. unfold Ord.suc. rewrite rLt_succ_iff. destruct H_rLt as [-> | ->].
+  - eapply Ord_join_l.
+  - eapply Ord_join_r.
+Qed.
+
+Lemma gtree_union_le_rev (X : Type@{Set_u}) (tr0 : gtree X) (tr1 : gtree X)
+  : Ord_join (@fromWf (gtree X) (@gtree_lt X) (gtree_lt_well_founded X) tr0) (@fromWf (gtree X) (@gtree_lt X) (gtree_lt_well_founded X) tr1) ≦ᵣ @fromWf (gtree X) (@gtree_lt X) (gtree_lt_well_founded X) (gtree_union tr0 tr1).
+Proof.
+  eapply Ord_join_spec; eapply rLt_implies_rLe; eapply member_implies_rLt; rewrite fromWf_unfold.
+  - exists tr0. split; [now left | reflexivity].
+  - exists tr1. split; [now right | reflexivity].
+Qed.
+
+Lemma gtree_top_O (X : Type@{Set_u})
+  : Ord.zer <ᵣ gtree_top X.
+Proof.
+  eapply rLe_rLt_rLt with (y := @fromWf (gtree X) (@gtree_lt X) (gtree_lt_well_founded X) gtree_O).
+  - exact (proj2 (gtree_O_rEq X)).
+  - eapply member_implies_rLt. exists gtree_O. reflexivity.
+Qed.
+
+Lemma gtree_top_S (X : Type@{Set_u}) (alpha : Ord.t)
+  (H_rLt : alpha <ᵣ gtree_top X)
+  : Ord.suc alpha <ᵣ gtree_top X.
+Proof.
+  destruct H_rLt as [[tr H_rLe]]. eapply rLe_rLt_rLt with (y := @fromWf (gtree X) (@gtree_lt X) (gtree_lt_well_founded X) (gtree_S tr)).
+  - transitivity (Ord.suc (@fromWf (gtree X) (@gtree_lt X) (gtree_lt_well_founded X) tr)).
+    + eapply Ord_suc_rLe. exact H_rLe.
+    + exact (proj2 (gtree_S_rEq X tr)).
+  - eapply member_implies_rLt. exists (gtree_S tr). reflexivity.
+Qed.
+
+Lemma gtree_top_union (X : Type@{Set_u}) (alpha : Ord.t) (beta : Ord.t)
+  (H_rLt0 : alpha <ᵣ gtree_top X)
+  (H_rLt1 : beta <ᵣ gtree_top X)
+  : Ord_join alpha beta <ᵣ gtree_top X.
+Proof.
+  destruct H_rLt0 as [[tr0 H_rLe0]], H_rLt1 as [[tr1 H_rLe1]].
+  eapply rLe_rLt_rLt with (y := @fromWf (gtree X) (@gtree_lt X) (gtree_lt_well_founded X) (gtree_union tr0 tr1)).
+  - transitivity (Ord_join (@fromWf (gtree X) (@gtree_lt X) (gtree_lt_well_founded X) tr0) (@fromWf (gtree X) (@gtree_lt X) (gtree_lt_well_founded X) tr1)).
+    + eapply Ord_join_spec.
+      * transitivity (@fromWf (gtree X) (@gtree_lt X) (gtree_lt_well_founded X) tr0); [exact H_rLe0 | eapply Ord_join_l].
+      * transitivity (@fromWf (gtree X) (@gtree_lt X) (gtree_lt_well_founded X) tr1); [exact H_rLe1 | eapply Ord_join_r].
+    + eapply gtree_union_le_rev.
+  - eapply member_implies_rLt. exists (gtree_union tr0 tr1). reflexivity.
+Qed.
+
+Lemma gtree_top_join (X : Type@{Set_u}) (P : X -> Prop) (os : @sig X P -> Ord.t)
+  (H_rLt : forall x : @sig X P, os x <ᵣ gtree_top X)
+  : Ord.sup (@sig X P) os <ᵣ gtree_top X.
+Proof.
+  pose proof (Axiom_of_Choice (@sig X P) (fun _ : @sig X P => gtree X) (fun x : @sig X P => fun tr : gtree X => os x ≦ᵣ @fromWf (gtree X) (@gtree_lt X) (gtree_lt_well_founded X) tr)) as [f H_f].
+  { intros x. pose proof (H_rLt x) as [[tr H_rLe]]. exists tr. exact H_rLe. }
+  eapply rLe_rLt_rLt with (y := @fromWf (gtree X) (@gtree_lt X) (gtree_lt_well_founded X) (gtree_join P f)).
+  - eapply Ord_sup_rLe_intro. intros x. transitivity (@fromWf (gtree X) (@gtree_lt X) (gtree_lt_well_founded X) (f x)).
+    + eapply H_f.
+    + eapply rLt_implies_rLe. eapply member_implies_rLt. rewrite fromWf_unfold. exists (f x). split; [now exists x | reflexivity].
+  - eapply member_implies_rLt. exists (gtree_join P f). reflexivity.
+Qed.
+
+Lemma gtree_top_S_ginaccessible (X : Type@{Set_u})
+  : ginaccessible X Ord.zer Ord.suc (gtree_top X).
+Proof.
+  econs.
+  - eapply gtree_top_O.
+  - eapply gtree_top_S.
+  - eapply gtree_top_join.
+  - eapply gtree_top_union.
+Qed.
+
+Lemma gtree_top_orec (X : Type@{Set_u}) (base0 : Ord.t) (next : Ord.t -> Ord.t) (base1 : Ord.t)
+  (H_next_le : forall alpha : Ord.t, alpha ≦ᵣ next alpha)
+  (H_next_mon : forall alpha : Ord.t, forall beta : Ord.t, alpha ≦ᵣ beta -> next alpha ≦ᵣ next beta)
+  (H_inaccessible : ginaccessible X base0 next (gtree_top X))
+  (H_base1 : base1 <ᵣ gtree_top X)
+  : forall alpha : Ord.t, alpha <ᵣ gtree_top X -> Ord.orec base1 next alpha <ᵣ gtree_top X.
+Proof.
+  intros alpha H_rLt.
+  enough (H_recs : forall tr : gtree X, Ord.orec base1 next (@fromWf (gtree X) (@gtree_lt X) (gtree_lt_well_founded X) tr) <ᵣ gtree_top X).
+  { destruct H_rLt as [[tr H_rLe]]. eapply rLe_rLt_rLt; [eapply Ord_orec_rLe; eauto; exact H_rLe | eapply H_recs]. }
+  intros tr. induction tr as [ | tr IH | P trs IH | tr0 IH0 tr1 IH1].
+  - eapply rLe_rLt_rLt with (y := base1).
+    + pose proof (Ord_orec_rEq_r base1 next (@fromWf (gtree X) (@gtree_lt X) (gtree_lt_well_founded X) gtree_O) Ord.zer H_next_le H_next_mon (gtree_O_rEq X)) as H_eq.
+      pose proof (Ord_orec_zer base1 next) as H_eq0. transitivity (Ord.orec base1 next Ord.zer).
+      * eapply H_eq.
+      * exact (proj1 H_eq0).
+    + exact H_base1.
+  - eapply rLe_rLt_rLt with (y := next (Ord.orec base1 next (@fromWf (gtree X) (@gtree_lt X) (gtree_lt_well_founded X) tr))).
+    + pose proof (Ord_orec_rEq_r base1 next (@fromWf (gtree X) (@gtree_lt X) (gtree_lt_well_founded X) (gtree_S tr)) (Ord.suc (@fromWf (gtree X) (@gtree_lt X) (gtree_lt_well_founded X) tr)) H_next_le H_next_mon (gtree_S_rEq X tr)) as H_eq.
+      transitivity (Ord.orec base1 next (Ord.suc (@fromWf (gtree X) (@gtree_lt X) (gtree_lt_well_founded X) tr))).
+      * eapply H_eq.
+      * exact (proj1 (Ord_orec_suc base1 next H_next_le H_next_mon (@fromWf (gtree X) (@gtree_lt X) (gtree_lt_well_founded X) tr))).
+    + eapply H_inaccessible. exact IH.
+  - eapply rLe_rLt_rLt with (y := Ord_join base1 (Ord.sup (@sig X P) (fun x : @sig X P => next (Ord.orec base1 next (@fromWf (gtree X) (@gtree_lt X) (gtree_lt_well_founded X) (trs x)))))).
+    + pose proof (Ord_orec_rEq_r base1 next (@fromWf (gtree X) (@gtree_lt X) (gtree_lt_well_founded X) (gtree_join P trs)) (mkNode (@sig X P) (fun x : @sig X P => @fromWf (gtree X) (@gtree_lt X) (gtree_lt_well_founded X) (trs x))) H_next_le H_next_mon (gtree_join_rEq X P trs)) as H_eq.
+      transitivity (Ord.orec base1 next (mkNode (@sig X P) (fun x : @sig X P => @fromWf (gtree X) (@gtree_lt X) (gtree_lt_well_founded X) (trs x)))).
+      * eapply H_eq.
+      * rewrite Ord_orec_unfold. reflexivity.
+    + eapply H_inaccessible.
+      * exact H_base1.
+      * eapply H_inaccessible. intros x. eapply H_inaccessible. exact (IH x).
+  - eapply rLe_rLt_rLt with (y := Ord.orec base1 next (Ord.suc (Ord_join (@fromWf (gtree X) (@gtree_lt X) (gtree_lt_well_founded X) tr0) (@fromWf (gtree X) (@gtree_lt X) (gtree_lt_well_founded X) tr1)))).
+    + eapply Ord_orec_rLe; eauto. eapply gtree_union_le.
+    + eapply rLe_rLt_rLt with (y := next (Ord.orec base1 next (Ord_join (@fromWf (gtree X) (@gtree_lt X) (gtree_lt_well_founded X) tr0) (@fromWf (gtree X) (@gtree_lt X) (gtree_lt_well_founded X) tr1)))).
+      * exact (proj1 (Ord_orec_suc base1 next H_next_le H_next_mon (Ord_join (@fromWf (gtree X) (@gtree_lt X) (gtree_lt_well_founded X) tr0) (@fromWf (gtree X) (@gtree_lt X) (gtree_lt_well_founded X) tr1)))).
+      * eapply H_inaccessible. eapply rLe_rLt_rLt with (y := Ord_join (Ord.orec base1 next (@fromWf (gtree X) (@gtree_lt X) (gtree_lt_well_founded X) tr0)) (Ord.orec base1 next (@fromWf (gtree X) (@gtree_lt X) (gtree_lt_well_founded X) tr1))).
+        { exact (proj1 (Ord_orec_join base1 next (@fromWf (gtree X) (@gtree_lt X) (gtree_lt_well_founded X) tr0) (@fromWf (gtree X) (@gtree_lt X) (gtree_lt_well_founded X) tr1) H_next_le H_next_mon)). }
+        { eapply H_inaccessible; assumption. }
+Qed.
+
+Lemma gtree_top_rec_ginaccessible (X : Type@{Set_u}) (base0 : Ord.t) (next : Ord.t -> Ord.t) (base1 : Ord.t)
+  (H_next_le : forall alpha : Ord.t, alpha ≦ᵣ next alpha)
+  (H_next_mon : forall alpha : Ord.t, forall beta : Ord.t, alpha ≦ᵣ beta -> next alpha ≦ᵣ next beta)
+  (H_inaccessible : ginaccessible X base0 next (gtree_top X))
+  (H_base1 : base1 <ᵣ gtree_top X)
+  : ginaccessible X base0 (Ord.orec base1 next) (gtree_top X).
+Proof.
+  econs.
+  - eapply H_inaccessible.
+  - eapply gtree_top_orec; eauto.
+  - eapply H_inaccessible.
+  - eapply H_inaccessible.
+Qed.
+
+Lemma gtree_top_add_ginaccessible (X : Type@{Set_u}) (alpha : Ord.t)
+  (H_rLt : alpha <ᵣ gtree_top X)
+  : ginaccessible X Ord.zer (Ord.add alpha) (gtree_top X).
+Proof.
+  unfold Ord.add. eapply gtree_top_rec_ginaccessible; eauto.
+  - intros x. eapply Ord_rLe_suc.
+  - intros x y H_rLe. eapply Ord_suc_rLe. exact H_rLe.
+  - eapply gtree_top_S_ginaccessible.
+Qed.
+
+Lemma gtree_top_add (X : Type@{Set_u}) (alpha : Ord.t) (beta : Ord.t)
+  (H_rLt0 : alpha <ᵣ gtree_top X)
+  (H_rLt1 : beta <ᵣ gtree_top X)
+  : Ord.add alpha beta <ᵣ gtree_top X.
+Proof.
+  eapply gtree_top_add_ginaccessible; eauto.
+Qed.
+
+Lemma gtree_top_flip_add_ginaccessible (X : Type@{Set_u}) (alpha : Ord.t)
+  (H_rLt : alpha <ᵣ gtree_top X)
+  : ginaccessible X Ord.zer (fun x : Ord.t => Ord.add x alpha) (gtree_top X).
+Proof.
+  econs.
+  - eapply gtree_top_O.
+  - intros x LT_x. eapply gtree_top_add; eauto.
+  - eapply gtree_top_join.
+  - eapply gtree_top_union.
+Qed.
+
+Lemma gtree_top_mul_ginaccessible (X : Type@{Set_u}) (alpha : Ord.t)
+  (H_rLt : alpha <ᵣ gtree_top X)
+  : ginaccessible X Ord.zer (Ord.mul alpha) (gtree_top X).
+Proof.
+  unfold Ord.mul. eapply gtree_top_rec_ginaccessible; eauto.
+  - intros x. eapply Ord_add_base_l.
+  - intros x y H_rLe. eapply Ord_add_rLe_l. exact H_rLe.
+  - eapply gtree_top_flip_add_ginaccessible. exact H_rLt.
+  - eapply gtree_top_O.
+Qed.
+
+Lemma gtree_top_mul (X : Type@{Set_u}) (alpha : Ord.t) (beta : Ord.t)
+  (H_rLt0 : alpha <ᵣ gtree_top X)
+  (H_rLt1 : beta <ᵣ gtree_top X)
+  : Ord.mul alpha beta <ᵣ gtree_top X.
+Proof.
+  eapply gtree_top_mul_ginaccessible; eauto.
+Qed.
+
+Lemma gtree_top_flip_mul_ginaccessible (X : Type@{Set_u}) (alpha : Ord.t)
+  (H_rLt : alpha <ᵣ gtree_top X)
+  : ginaccessible X Ord.zer (fun x : Ord.t => Ord.mul x alpha) (gtree_top X).
+Proof.
+  econs.
+  - eapply gtree_top_O.
+  - intros x LT_x. eapply gtree_top_mul; eauto.
+  - eapply gtree_top_join.
+  - eapply gtree_top_union.
+Qed.
+
+Lemma gtree_top_exp_ginaccessible (X : Type@{Set_u}) (alpha : Ord.t)
+  (H_pos : Ord.zer <ᵣ alpha)
+  (H_rLt : alpha <ᵣ gtree_top X)
+  : ginaccessible X Ord.zer (Ord.exp alpha) (gtree_top X).
+Proof.
+  unfold Ord.exp. eapply gtree_top_rec_ginaccessible; eauto.
+  - intros x. eapply Ord_mul_base_l. exact H_pos.
+  - intros x y H_rLe. eapply Ord_mul_rLe_l. exact H_rLe.
+  - eapply gtree_top_flip_mul_ginaccessible. exact H_rLt.
+  - unfold Ord.one. eapply gtree_top_S. eapply gtree_top_O.
+Qed.
+
+Lemma gtree_top_exp (X : Type@{Set_u}) (alpha : Ord.t) (beta : Ord.t)
+  (H_rLt0 : alpha <ᵣ gtree_top X)
+  (H_rLt1 : beta <ᵣ gtree_top X)
+  : Ord.exp alpha beta <ᵣ gtree_top X.
+Proof.
+  eapply rLe_rLt_rLt with (y := Ord.exp (Ord.suc alpha) beta).
+  - eapply Ord_exp_rLe_l. eapply Ord_rLe_suc.
+  - eapply gtree_top_exp_ginaccessible.
+    + eapply rLe_rLt_rLt with (y := alpha); [eapply Ord_zer_rLe | unfold Ord.suc; eapply rLt_succ_intro].
+    + eapply gtree_top_S. exact H_rLt0.
+    + exact H_rLt1.
+Qed.
+
+Lemma gtree_top_flip_exp_ginaccessible (X : Type@{Set_u}) (alpha : Ord.t)
+  (H_rLt : alpha <ᵣ gtree_top X)
+  : ginaccessible X Ord.zer (fun x : Ord.t => Ord.exp x alpha) (gtree_top X).
+Proof.
+  econs.
+  - eapply gtree_top_O.
+  - intros x LT_x. eapply gtree_top_exp; eauto.
+  - eapply gtree_top_join.
+  - eapply gtree_top_union.
+Qed.
+
+Definition kappa : Ord.t :=
+  @mkNode { A : Type & { R : A -> A -> Prop | well_founded R } } (fun RWF => @fromWfSet (projT1 RWF) (proj1_sig (projT2 RWF)) (proj2_sig (projT2 RWF))).
+
+Lemma kappa_complete (alpha : Ord.t)
+  (H_rLt : alpha <ᵣ kappa)
+  : exists A : Type, exists R : A -> A -> Prop, exists R_wf : well_founded R, alpha ≦ᵣ @fromWfSet A R R_wf.
+Proof.
+  destruct H_rLt as [[[A [R R_wf]] H_rLe]]. exists A, R, R_wf. exact H_rLe.
+Qed.
+
+Lemma kappa_inaccessible_from_wf_set (A : Type) (R : A -> A -> Prop) (R_wf : well_founded R)
+  : @fromWfSet A R R_wf <ᵣ kappa.
+Proof.
+  econs. exists (@existT Type (fun A : Type => { R : A -> A -> Prop | well_founded R }) A (@exist (A -> A -> Prop) (@well_founded A) R R_wf)). reflexivity.
+Qed.
+
+Lemma kappa_inaccessible_from_wf (A : Type) (R : A -> A -> Prop) (R_wf : well_founded R) (a : A)
+  : @fromWf A R R_wf a <ᵣ kappa.
+Proof.
+  eapply rLt_rLe_rLt with (y := @fromWfSet A R R_wf).
+  - eapply member_implies_rLt. exists a. reflexivity.
+  - eapply rLt_implies_rLe. eapply kappa_inaccessible_from_wf_set.
+Qed.
+
+Lemma kappa_inaccessible_cardinality (A : Type)
+  : Cardinality.toTree (Cardinality.ofType A) <ᵣ kappa.
+Proof.
+  pose proof (well_ordering_thm A (@mkSetoid_from_eq A)) as (R & R_wf & R_total & R_trans & R_compat).
+  eapply rLe_rLt_rLt with (y := @fromWfSet A R R_wf).
+  - eapply Cardinal1.Cardinality_lowerbound; eauto.
+  - eapply kappa_inaccessible_from_wf_set.
+Qed.
+
+Lemma kappa_inaccessible_O
+  : Ord.zer <ᵣ kappa.
+Proof.
+  eapply rLe_rLt_rLt with (y := @fromWfSet Empty_set (fun x : Empty_set => fun _ : Empty_set => False) (Empty_set_ind _)).
+  - eapply Ord_zer_rLe.
+  - eapply kappa_inaccessible_from_wf_set.
+Qed.
+
+Lemma kappa_inaccessible_is_S (alpha : Ord.t) (beta : Ord.t)
+  (H_succ : beta =ᵣ Ord.suc alpha)
+  (H_rLt : alpha <ᵣ kappa)
+  : beta <ᵣ kappa.
+Proof.
+  rewrite H_succ. pose proof (kappa_complete alpha H_rLt) as (A & R & R_wf & H_rLe).
+  set (Ropt := fun x : option A => fun y : option A =>
+    match x, y with
+    | Some x', Some y' => R x' y'
+    | Some x', None => True
+    | None, _ => False
+    end
+  ).
+  assert (H_some_acc : forall a : A, Acc Ropt (Some a)).
+  { intros a. induction (R_wf a) as [a H_Acc_inv IH]. econs. intros [b | ] H_rel.
+    - eapply IH. exact H_rel.
+    - contradiction.
+  }
+  assert (Ropt_wf : well_founded Ropt).
+  { intros [a | ]. eapply H_some_acc. econs. intros [a | ] H_rel.
+    - eapply H_some_acc.
+    - contradiction.
+  }
+  assert (H_top : @fromWfSet A R R_wf ≦ᵣ @fromWf (option A) Ropt Ropt_wf None).
+  { econs. intros a.
+    assert (H_rLe_a : @fromWf A R R_wf a ≦ᵣ @fromWf (option A) Ropt Ropt_wf (Some a)).
+    { eapply fromWf_cong with (RA := R) (RB := Ropt) (f := @Some A) (RA_wf := R_wf) (RB_wf := Ropt_wf). intros x y H_xy. exact H_xy. }
+    assert (H_rLt_a : @fromWf (option A) Ropt Ropt_wf (Some a) <ᵣ @fromWf (option A) Ropt Ropt_wf None).
+    { eapply member_implies_rLt. rewrite fromWf_unfold. exists (Some a). split; [reflexivity | reflexivity]. }
+    eapply rLe_rLt_rLt; eauto.
+  }
+  eapply rLe_rLt_rLt with (y := Ord.suc (@fromWfSet A R R_wf)).
+  - eapply Ord_suc_rLe. exact H_rLe.
+  - eapply rLe_rLt_rLt with (y := @fromWfSet (option A) Ropt Ropt_wf).
+    + unfold Ord.suc. rewrite succ_rLe_iff. eapply rLe_rLt_rLt with (y := @fromWf (option A) Ropt Ropt_wf None).
+      * exact H_top.
+      * eapply member_implies_rLt. exists None. reflexivity.
+    + eapply kappa_inaccessible_from_wf_set.
+Qed.
+
+Lemma kappa_inaccessible_S (alpha : Ord.t)
+  (H_rLt : alpha <ᵣ kappa)
+  : Ord.suc alpha <ᵣ kappa.
+Proof.
+  eapply kappa_inaccessible_is_S; eauto. reflexivity.
+Qed.
+
+Lemma kappa_inaccessible_Ord_of_nat (n : nat)
+  : Ord_of_nat n <ᵣ kappa.
+Proof.
+  induction n as [ | n IH].
+  - eapply kappa_inaccessible_O.
+  - simpl. eapply kappa_inaccessible_S. exact IH.
+Qed.
+
+Lemma kappa_inaccessible_join (A : Type) (os : A -> Ord.t)
+  (H_rLt : forall a : A, os a <ᵣ kappa)
+  : Ord.sup A os <ᵣ kappa.
+Proof.
+  pose proof (Axiom_of_Choice A (fun _ : A => { B : Type & { R : B -> B -> Prop | well_founded R } }) (fun a : A => fun RWF : { B : Type & { R : B -> B -> Prop | well_founded R } } => os a ≦ᵣ @fromWfSet (projT1 RWF) (proj1_sig (projT2 RWF)) (proj2_sig (projT2 RWF)))) as [f H_f].
+  { intros a. pose proof (kappa_complete (os a) (H_rLt a)) as (B & R & R_wf & H_rLe). exists (@existT Type (fun B : Type => { R : B -> B -> Prop | well_founded R }) B (@exist (B -> B -> Prop) (@well_founded B) R R_wf)). exact H_rLe. }
+  set (B := fun a : A => projT1 (f a)).
+  set (R := fun a : A => proj1_sig (projT2 (f a))).
+  set (R_wf := fun a : A => proj2_sig (projT2 (f a))).
+  pose (A_join := { a : A & option (B a) }).
+  pose (fun x : A_join => fun y : A_join =>
+    match y with
+    | @existT _ _ a None =>
+      match x with
+      | @existT _ _ a' (Some _) => a = a'
+      | _ => False
+      end
+    | @existT _ _ a (Some y') =>
+      match x with
+      | @existT _ _ a' (Some x') => exists H_eq : a' = a, R a (eq_rect a' B x' a H_eq) y'
+      | _ => False
+      end
+    end
+  ) as R_join.
+  assert (R_join_wf : well_founded R_join).
+  { intros [a [x | ]].
+    + induction (R_wf a x) as [x H_Acc_inv IH]. econs. intros [a' [y | ]] H_rel.
+      * unfold R_join in H_rel. destruct H_rel as [H_eq H_rel]. subst a'. simpl in H_rel. eapply IH. exact H_rel.
+      * contradiction.
+    + econs. intros [a' [y | ]] H_rel.
+      * unfold R_join in H_rel. subst a'. induction (R_wf a y) as [y H_Acc_inv IH]. econs. intros [a' [z | ]] H_rel.
+        { unfold R_join in H_rel. destruct H_rel as [H_eq H_rel]. subst a'. simpl in H_rel. eapply IH. exact H_rel. }
+        { contradiction. }
+      * contradiction.
+  }
+  eapply rLe_rLt_rLt with (y := @fromWfSet A_join R_join R_join_wf).
+  - eapply Ord_sup_rLe_intro. intros a. transitivity (@fromWfSet (B a) (R a) (R_wf a)).
+    + eapply H_f.
+    + eapply rLt_implies_rLe. eapply rLe_rLt_rLt with (y := @fromWf A_join R_join R_join_wf (@existT A (fun a : A => option (B a)) a None)).
+      * econs. intros x. eapply rLe_rLt_rLt with (y := @fromWf A_join R_join R_join_wf (@existT A (fun a : A => option (B a)) a (Some x))).
+        { eapply fromWf_cong with (RA := R a) (RB := R_join) (f := fun x : B a => @existT A (fun a : A => option (B a)) a (Some x)) (RA_wf := R_wf a) (RB_wf := R_join_wf). intros x0 y0 H_xy. exists eq_refl. exact H_xy. }
+        { eapply member_implies_rLt. rewrite fromWf_unfold. exists (@existT A (fun a : A => option (B a)) a (Some x)). split; [reflexivity | reflexivity]. }
+      * eapply member_implies_rLt. exists (@existT A (fun a : A => option (B a)) a None). reflexivity.
+  - eapply kappa_inaccessible_from_wf_set.
+Qed.
+
+Lemma kappa_inaccessible_union (alpha : Ord.t) (beta : Ord.t)
+  (H_rLt : alpha <ᵣ kappa)
+  (H_rLt' : beta <ᵣ kappa)
+  : Ord_join alpha beta <ᵣ kappa.
+Proof.
+  unfold Ord_join. eapply kappa_inaccessible_join. intros [ | ]; assumption.
+Qed.
+
+Lemma kappa_inaccessible_omega
+  : omega <ᵣ kappa.
+Proof.
+  unfold omega. eapply kappa_inaccessible_join. intros n. eapply kappa_inaccessible_Ord_of_nat.
+Qed.
+
+Lemma kappa_inaccessible_orec (base : Ord.t) (next : Ord.t -> Ord.t)
+  (H_next_le : forall alpha : Ord.t, alpha ≦ᵣ next alpha)
+  (H_next_mon : forall alpha : Ord.t, forall beta : Ord.t, alpha ≦ᵣ beta -> next alpha ≦ᵣ next beta)
+  (H_base : base <ᵣ kappa)
+  (H_next : forall alpha : Ord.t, alpha <ᵣ kappa -> next alpha <ᵣ kappa)
+  : forall alpha : Ord.t, alpha <ᵣ kappa -> Ord.orec base next alpha <ᵣ kappa.
+Proof.
+  intros alpha H_rLt.
+  pose proof (kappa_complete alpha H_rLt) as (A & R & R_wf & H_rLe).
+  assert (H_rec : forall a : A, Ord.orec base next (@fromWf A R R_wf a) <ᵣ kappa).
+  { intros a. induction (R_wf a) as [a H_Acc_inv IH].
+    eapply rLe_rLt_rLt with (y := Ord.orec base next (Ord.suc (Ord.sup (@sig A (fun b : A => R b a)) (fun b : @sig A (fun b : A => R b a) => @fromWf A R R_wf (proj1_sig b))))).
+    - eapply Ord_orec_rLe; eauto. eapply fromWf_isSupremum. intros b R_b_a.
+      eapply rLe_rLt_rLt with (y := Ord.sup (@sig A (fun b : A => R b a)) (fun b : @sig A (fun b : A => R b a) => @fromWf A R R_wf (proj1_sig b))).
+      + change ((fun b0 : @sig A (fun b : A => R b a) => @fromWf A R R_wf (proj1_sig b0)) (@exist A (fun b : A => R b a) b R_b_a) ≦ᵣ Ord.sup (@sig A (fun b : A => R b a)) (fun b0 : @sig A (fun b : A => R b a) => @fromWf A R R_wf (proj1_sig b0))). eapply Ord_rLe_sup_intro.
+      + unfold Ord.suc. eapply rLt_succ_intro.
+    - eapply rLe_rLt_rLt with (y := next (Ord.orec base next (Ord.sup (@sig A (fun b : A => R b a)) (fun b : @sig A (fun b : A => R b a) => @fromWf A R R_wf (proj1_sig b))))).
+      + exact (proj1 (Ord_orec_suc base next H_next_le H_next_mon (Ord.sup (@sig A (fun b : A => R b a)) (fun b : @sig A (fun b : A => R b a) => @fromWf A R R_wf (proj1_sig b))))).
+      + eapply H_next. eapply rLe_rLt_rLt with (y := Ord_join base (Ord.sup (@sig A (fun b : A => R b a)) (fun b : @sig A (fun b : A => R b a) => Ord.orec base next (@fromWf A R R_wf (proj1_sig b))))).
+        * exact (proj1 (Ord_orec_sup base next (@sig A (fun b : A => R b a)) (fun b : @sig A (fun b : A => R b a) => @fromWf A R R_wf (proj1_sig b)) H_next_le H_next_mon)).
+        * eapply kappa_inaccessible_union.
+          { exact H_base. }
+          { eapply kappa_inaccessible_join. intros [b R_b_a]. eapply IH. exact R_b_a. }
+  }
+  eapply rLe_rLt_rLt with (y := Ord.orec base next (@fromWfSet A R R_wf)).
+  - eapply Ord_orec_rLe; [exact H_next_le | exact H_next_mon | exact H_rLe].
+  - eapply rLe_rLt_rLt with (y := Ord_join base (Ord.sup A (fun a : A => next (Ord.orec base next (@fromWf A R R_wf a))))).
+    + unfold fromWfSet. rewrite Ord_orec_unfold. reflexivity.
+    + eapply kappa_inaccessible_union.
+      * exact H_base.
+      * eapply kappa_inaccessible_join. intros a. eapply H_next. eapply H_rec.
+Qed.
+
+Lemma kappa_inaccessible_add (alpha : Ord.t) (beta : Ord.t)
+  (H_rLt0 : alpha <ᵣ kappa)
+  (H_rLt1 : beta <ᵣ kappa)
+  : Ord.add alpha beta <ᵣ kappa.
+Proof.
+  unfold Ord.add. eapply kappa_inaccessible_orec; eauto.
+  - intros x. eapply Ord_rLe_suc.
+  - intros x y H_rLe. eapply Ord_suc_rLe. exact H_rLe.
+  - intros x H_rLt. eapply kappa_inaccessible_S. exact H_rLt.
+Qed.
+
+Lemma kappa_inaccessible_mul (alpha : Ord.t) (beta : Ord.t)
+  (H_rLt0 : alpha <ᵣ kappa)
+  (H_rLt1 : beta <ᵣ kappa)
+  : Ord.mul alpha beta <ᵣ kappa.
+Proof.
+  unfold Ord.mul. eapply kappa_inaccessible_orec; eauto.
+  - intros x. eapply Ord_add_base_l.
+  - intros x y H_rLe. eapply Ord_add_rLe_l. exact H_rLe.
+  - eapply kappa_inaccessible_O.
+  - intros x H_rLt. eapply kappa_inaccessible_add; eauto.
+Qed.
+
+Lemma kappa_inaccessible_exp (alpha : Ord.t) (beta : Ord.t)
+  (H_rLt0 : alpha <ᵣ kappa)
+  (H_rLt1 : beta <ᵣ kappa)
+  : Ord.exp alpha beta <ᵣ kappa.
+Proof.
+  eapply rLe_rLt_rLt with (y := Ord.exp (Ord.suc alpha) beta).
+  - eapply Ord_exp_rLe_l. eapply Ord_rLe_suc.
+  - unfold Ord.exp. eapply kappa_inaccessible_orec; eauto.
+    + intros x. eapply Ord_mul_base_l. eapply rLe_rLt_rLt with (y := alpha).
+      * eapply Ord_zer_rLe.
+      * unfold Ord.suc. eapply rLt_succ_intro.
+    + intros x y H_rLe. eapply Ord_mul_rLe_l. exact H_rLe.
+    + unfold Ord.one. eapply kappa_inaccessible_S. eapply kappa_inaccessible_O.
+    + intros x H_rLt. eapply kappa_inaccessible_mul.
+      * exact H_rLt.
+      * eapply kappa_inaccessible_S. exact H_rLt0.
+Qed.
+
+End CLASSICAL.
+
+End Inaccessible.
