theories/Prelude/Notations.v
@@ -1,5 +1,6 @@
 Require Import PnV.Prelude.SfLib.
 
+Reserved Infix "≝" (no associativity, at level 100).
 Reserved Infix "==" (no associativity, at level 70).
 Reserved Infix "≡" (no associativity, at level 70).
 Reserved Infix "≡ₐ" (no associativity, at level 70).
@@ -33,6 +34,8 @@ Reserved Infix "\subseteq" (no associativity, at level 70).
 
 Reserved Infix "∈" (no associativity, at level 70).
 Reserved Infix "⊆" (no associativity, at level 70).
+Reserved Infix "∉" (no associativity, at level 70).
+Reserved Infix "∌" (no associativity, at level 70).
 
 Reserved Infix "⊢" (no associativity, at level 70).
 Reserved Infix "⊨" (no associativity, at level 70).
